finish all proofs about properties of cache

src/newBBCache/CompCache.v
@@ -8,15 +8,8 @@ Set Implicit Arguments.
 Unset Strict Implicit.
 Import Prenex Implicits.
 
-(* Module ExpMap <: SsrFMap := FMaps.MakeTreeMap QFBV.ExpOrder. *)
-(* Module BexpMap <: SsrFMap := FMaps.MakeTreeMap QFBV.BexpOrder. *)
 
-(* Definition cexpm := ExpMap.t (cnf * word). *)
-(* Definition cbexpm := BexpMap.t (cnf * literal). *)
-(* Definition hexpm := ExpMap.t (cnf * word). *)
-(* Definition hbexpm := BexpMap.t (cnf * literal). *)
-
-(* ==== A cache with complete information in both current and historical tables ==== *)
+(* == A cache with complete information in both current and historical tables == *)
 
 Record compcache :=
   { (* store historical results *)
@@ -24,75 +17,75 @@ Record compcache :=
     (* store current results *)
     ct : comptable }.
 
-Definition find_het e c := find_et e (ht c).
-Definition find_hbt e c := find_bt e (ht c). 
-Definition find_cet e c := find_et e (ct c). 
-Definition find_cbt e c := find_bt e (ct c). 
+Definition empty : compcache :=
+  {| ht := CompTable.empty;
+     ct := CompTable.empty |}.
 
-(* Definition get_het e c := *)
-(*   match find_het e c with *)
-(*   | Some (cs, ls) => (cs, ls) *)
-(*   | None => ([::], [::lit_tt]) (* default value, in fact never used *) *)
-(*   end. *)
-
-(* Definition get_hbt e c := *)
-(*   match find_hbt e c with *)
-(*   | Some (cs, l) => (cs, l) *)
-(*   | None => ([::], lit_tt) (* default value, in fact never used *) *)
-(*   end. *)
+Definition find_het e c := CompTable.find_et e (ht c).
+Definition find_hbt e c := CompTable.find_bt e (ht c). 
+Definition find_cet e c := CompTable.find_et e (ct c). 
+Definition find_cbt e c := CompTable.find_bt e (ct c). 
 
 
-(* Definition find_cnf_exp e c := *)
-(*   match find_het e c with *)
-(*   | None => [::] *)
-(*   | Some (cs, ls) => cs *)
-(*   end. *)
-(* Definition find_cnf_bexp e c := *)
-(*   match find_hbt e c with *)
-(*   | None => [::] *)
-(*   | Some (cs, l) => cs *)
-(*   end. *)
-(* Definition find_lits_exp e c := *)
-(*   match find_het e c with *)
-(*   | None => [::lit_tt] *)
-(*   | Some (cs, ls) => ls *)
-(*   end. *)
-(* Definition find_lit_bexp e c := *)
-(*   match find_hbt e c with *)
-(*   | None => lit_tt *)
-(*   | Some (cs, l) => l *)
-(*   end. *)
+(* ==== modification ==== *)
 
 Definition add_het e cs ls c := 
-  {| ht := add_et e cs ls (ht c);
+  {| ht := CompTable.add_et e cs ls (ht c);
      ct := ct c |}.
+
 Definition add_hbt e cs l c := 
-  {| ht := add_bt e cs l (ht c);
+  {| ht := CompTable.add_bt e cs l (ht c);
      ct := ct c |}.
+
 Definition add_cet e cs ls c := 
   {| ht := ht c;
-     ct := add_et e cs ls (ct c) |}.
+     ct := CompTable.add_et e cs ls (ct c) |}.
+
 Definition add_cbt e cs l c := 
   {| ht := ht c;
-     ct := add_bt e cs l (ct c) |}.
+     ct := CompTable.add_bt e cs l (ct c) |}.
 
 Definition reset_ct (c : compcache) :=
   {| ht := ht c;
-     ct := {| et := ExpMap.empty (cnf * word);
-              bt := BexpMap.empty (cnf * literal) |} |}.
+     ct := CompTable.empty |}.
+
+Lemma add_het_cet_comm :
+  forall c e1 cs1 ls1 e2 cs2 ls2,
+    add_het e1 cs1 ls1 (add_cet e2 cs2 ls2 c) 
+    = add_cet e2 cs2 ls2 (add_het e1 cs1 ls1 c).
+Proof.
+  done.
+Qed.
+
+Lemma add_het_cbt_comm :
+  forall c e1 cs1 ls1 e2 cs2 l2,
+    add_het e1 cs1 ls1 (add_cbt e2 cs2 l2 c) 
+    = add_cbt e2 cs2 l2 (add_het e1 cs1 ls1 c).
+Proof.
+  done.
+Qed.
+
+Lemma add_hbt_cet_comm :
+  forall c e1 cs1 l1 e2 cs2 ls2,
+    add_hbt e1 cs1 l1 (add_cet e2 cs2 ls2 c) 
+    = add_cet e2 cs2 ls2 (add_hbt e1 cs1 l1 c).
+Proof.
+  done.
+Qed.
+
+Lemma add_hbt_cbt_comm :
+  forall c e1 cs1 l1 e2 cs2 l2,
+    add_hbt e1 cs1 l1 (add_cbt e2 cs2 l2 c) 
+    = add_cbt e2 cs2 l2 (add_hbt e1 cs1 l1 c).
+Proof.
+  done.
+Qed.
 
 Lemma find_het_add_het_eq :
   forall e cs ls c, find_het e (add_het e cs ls c) = Some (cs, ls).
 Proof.
   move=> e cs ls c. rewrite /find_het /add_het /=. 
   by apply: CompTable.find_et_add_et_eq.
-Qed.
-
-Lemma find_hbt_add_hbt_eq :
-  forall e cs l c, find_hbt e (add_hbt e cs l c) = Some (cs, l).
-Proof.
-  move=> e cs l c. rewrite /find_hbt /add_hbt /=. 
-  by apply: CompTable.find_bt_add_bt_eq.
 Qed.
 
 Lemma find_het_add_het_neq :
@@ -102,18 +95,23 @@ Proof.
   by apply: CompTable.find_et_add_et_neq.
 Qed.
 
-Lemma find_hbt_add_hbt_neq :
-  forall e0 e cs l c, ~ e0 == e -> find_hbt e0 (add_hbt e cs l c) = find_hbt e0 c.
-Proof.
-  move=> e0 e cs l c. rewrite /find_hbt /add_hbt /=.
-  by apply: CompTable.find_bt_add_bt_neq.
-Qed.
-
 Lemma find_het_add_hbt :
   forall e0 e cs l c, find_het e0 (add_hbt e cs l c) = find_het e0 c.
 Proof.
   move=> e0 e cs l c. rewrite /find_het /add_hbt /=.
   by apply: CompTable.find_et_add_bt.
+Qed.
+
+Lemma find_het_add_cet :
+  forall e0 e cs ls c, find_het e0 (add_cet e cs ls c) = find_het e0 c.
+Proof.
+  done.
+Qed.
+
+Lemma find_het_add_cbt :
+  forall e0 e cs l c, find_het e0 (add_cbt e cs l c) = find_het e0 c.
+Proof.
+  done.
 Qed.
 
 Lemma find_hbt_add_het :
@@ -123,18 +121,49 @@ Proof.
   by apply: CompTable.find_bt_add_et.
 Qed.
 
+Lemma find_hbt_add_hbt_eq :
+  forall e cs l c, find_hbt e (add_hbt e cs l c) = Some (cs, l).
+Proof.
+  move=> e cs l c. rewrite /find_hbt /add_hbt /=. 
+  by apply: CompTable.find_bt_add_bt_eq.
+Qed.
+
+Lemma find_hbt_add_hbt_neq :
+  forall e0 e cs l c, ~ e0 == e -> find_hbt e0 (add_hbt e cs l c) = find_hbt e0 c.
+Proof.
+  move=> e0 e cs l c. rewrite /find_hbt /add_hbt /=.
+  by apply: CompTable.find_bt_add_bt_neq.
+Qed.
+
+Lemma find_hbt_add_cet :
+  forall e0 e cs ls c, find_hbt e0 (add_cet e cs ls c) = find_hbt e0 c.
+Proof.
+  done.
+Qed.
+
+Lemma find_hbt_add_cbt :
+  forall e0 e cs l c, find_hbt e0 (add_cbt e cs l c) = find_hbt e0 c.
+Proof.
+  done.
+Qed.
+
+Lemma find_cet_add_het :
+  forall e0 e cs ls c, find_cet e0 (add_het e cs ls c) = find_cet e0 c.
+Proof.
+  done.
+Qed.
+
+Lemma find_cet_add_hbt :
+  forall e0 e cs l c, find_cet e0 (add_hbt e cs l c) = find_cet e0 c.
+Proof.
+  done.
+Qed.
+
 Lemma find_cet_add_cet_eq :
   forall e cs ls c, find_cet e (add_cet e cs ls c) = Some (cs, ls).
 Proof.
   move=> e cs ls c. rewrite /find_cet /add_cet /=. 
   by apply: CompTable.find_et_add_et_eq.
-Qed.
-
-Lemma find_cbt_add_cbt_eq :
-  forall e cs l c, find_cbt e (add_cbt e cs l c) = Some (cs, l).
-Proof.
-  move=> e cs l c. rewrite /find_cbt /add_cbt /=. 
-  by apply: CompTable.find_bt_add_bt_eq.
 Qed.
 
 Lemma find_cet_add_cet_neq :
@@ -144,18 +173,23 @@ Proof.
   by apply: CompTable.find_et_add_et_neq.
 Qed.
 
-Lemma find_cbt_add_cbt_neq :
-  forall e0 e cs l c, ~ e0 == e -> find_cbt e0 (add_cbt e cs l c) = find_cbt e0 c.
-Proof.
-  move=> e0 e cs l c. rewrite /find_cbt /add_cbt /=.
-  by apply: CompTable.find_bt_add_bt_neq.
-Qed.
-
 Lemma find_cet_add_cbt :
   forall e0 e cs l c, find_cet e0 (add_cbt e cs l c) = find_cet e0 c.
 Proof.
   move=> e0 e cs l c. rewrite /find_cet /add_cbt /=.
   by apply: CompTable.find_et_add_bt.
+Qed.
+
+Lemma find_cbt_add_het :
+  forall e0 e cs ls c, find_cbt e0 (add_het e cs ls c) = find_cbt e0 c.
+Proof.
+  done.
+Qed.
+
+Lemma find_cbt_add_hbt :
+  forall e0 e cs l c, find_cbt e0 (add_hbt e cs l c) = find_cbt e0 c.
+Proof.
+  done.
 Qed.
 
 Lemma find_cbt_add_cet :
@@ -165,134 +199,205 @@ Proof.
   by apply: CompTable.find_bt_add_et.
 Qed.
 
-Lemma find_cet_add_het :
-  forall e0 e cs ls c, find_cet e0 (add_het e cs ls c) = find_cet e0 c.
+Lemma find_cbt_add_cbt_eq :
+  forall e cs l c, find_cbt e (add_cbt e cs l c) = Some (cs, l).
 Proof.
-Admitted.
-
-Lemma find_cet_add_hbt :
-  forall e0 e cs l c, find_cet e0 (add_hbt e cs l c) = find_cet e0 c.
-Proof.
-Admitted.
-
-Lemma find_het_add_cet :
-  forall e0 e cs ls c, find_het e0 (add_cet e cs ls c) = find_het e0 c.
-Proof.
-Admitted.
-
-Lemma find_het_add_cbt :
-  forall e0 e cs l c, find_het e0 (add_cbt e cs l c) = find_het e0 c.
-Proof.
-Admitted.
-
-
-
-
-
-
-(*
-Lemma find_cnf_exp_add_het_eq :
-  forall e cs ls c, find_cnf_exp e (add_het e cs ls c) = cs.
-Proof.
-  move=> e cs ls c. rewrite /find_cnf_exp find_het_add_het_eq. done.
+  move=> e cs l c. rewrite /find_cbt /add_cbt /=. 
+  by apply: CompTable.find_bt_add_bt_eq.
 Qed.
 
-Lemma find_lits_exp_add_het_eq :
-  forall e cs ls c, find_lits_exp e (add_het e cs ls c) = ls.
+Lemma find_cbt_add_cbt_neq :
+  forall e0 e cs l c, ~ e0 == e -> find_cbt e0 (add_cbt e cs l c) = find_cbt e0 c.
 Proof.
-  move=> e cs ls c. rewrite /find_lits_exp find_het_add_het_eq. done.
+  move=> e0 e cs l c. rewrite /find_cbt /add_cbt /=.
+  by apply: CompTable.find_bt_add_bt_neq.
 Qed.
-
-Lemma find_cnf_bexp_add_hbt_eq :
-  forall e cs l c, find_cnf_bexp e (add_hbt e cs l c) = cs.
-Proof.
-  move=> e cs l c. rewrite /find_cnf_bexp find_hbt_add_hbt_eq. done.
-Qed.
-
-Lemma find_lit_bexp_add_hbt_eq :
-  forall e cs l c, find_lit_bexp e (add_hbt e cs l c) = l.
-Proof.
-  move=> e cs l c. rewrite /find_lit_bexp find_hbt_add_hbt_eq. done.
-Qed.
-*)
 
 
 (* ==== well_formed ==== *)
 
 Definition well_formed (c : compcache) : Prop := 
-  (forall e cs ls, find_cet e c = Some (cs, ls)
-                   -> find_het e c = Some (cs, ls))
-  /\ forall e cs l, find_cbt e c = Some (cs, l)
-                    -> find_hbt e c = Some (cs, l).
+  (forall e cs ls, find_cet e c = Some (cs, ls) -> find_het e c = Some (cs, ls))
+  /\ forall e cs l, find_cbt e c = Some (cs, l) -> find_hbt e c = Some (cs, l).
 
 Lemma well_formed_find_cet :
   forall c e cs ls,
     well_formed c -> find_cet e c = Some (cs, ls) -> find_het e c = Some (cs, ls).
-Proof. Admitted.
+Proof. 
+  move=> c e cs ls [He Hb]. exact: He.
+Qed.
 
 Lemma well_formed_find_cbt :
   forall c e cs l,
     well_formed c -> find_cbt e c = Some (cs, l) -> find_hbt e c = Some (cs, l).
-Proof. Admitted.
+Proof.
+  move=> c e cs l [He Hb]. exact: Hb.
+Qed.
 
 Lemma well_formed_add_cet :
   forall c e cs ls,
     well_formed c -> find_het e c = Some (cs, ls) -> well_formed (add_cet e cs ls c).
-Proof. Admitted.
+Proof. 
+  move=> c e1 cs1 ls1 Hwfc Hfhete1. split.
+  - move=> e2 cs2 ls2. case Heq : (e2 == e1).
+    + move/eqP: Heq => ->. rewrite find_cet_add_cet_eq. case=> <- <-.
+      rewrite find_het_add_cet. done.
+    + move/negP: Heq => Hneq. rewrite (find_cet_add_cet_neq _ _ _ Hneq) => Hfcete2.
+      rewrite find_het_add_cet. exact: (well_formed_find_cet Hwfc Hfcete2).
+  - move=> e2 cs2 l2. rewrite find_cbt_add_cet find_hbt_add_cet.
+    move=> Hfcbte2. exact: (well_formed_find_cbt Hwfc Hfcbte2).
+Qed.
 
 Lemma well_formed_add_cbt :
   forall c e cs l,
     well_formed c -> find_hbt e c = Some (cs, l) -> well_formed (add_cbt e cs l c).
-Proof. Admitted.
+Proof.
+  move=> c e1 cs1 l1 Hwfc Hfhbte1. split.
+  - move=> e2 cs2 ls2. rewrite find_cet_add_cbt find_het_add_cbt.
+    move=> Hfcete2. exact: (well_formed_find_cet Hwfc Hfcete2).
+  - move=> e2 cs2 l2. case Heq : (e2 == e1).
+    + move/eqP: Heq => ->. rewrite find_cbt_add_cbt_eq. case=> <- <-.
+      rewrite find_hbt_add_cbt. done.
+    + move/negP: Heq => Hneq. rewrite (find_cbt_add_cbt_neq _ _ _ Hneq) => Hfcbte2.
+      rewrite find_hbt_add_cbt. exact: (well_formed_find_cbt Hwfc Hfcbte2).
+Qed.
 
 Lemma well_formed_add_cet_het :
   forall c e cs ls,
     well_formed c -> well_formed (add_cet e cs ls (add_het e cs ls c)).
-Proof. Admitted.
+Proof.
+  move=> c e1 cs1 ls1 Hwfc. split.
+  - move=> e2 cs2 ls2. case Heq : (e2 == e1).
+    + move/eqP: Heq => ->. rewrite find_cet_add_cet_eq. case=> <- <-.
+      rewrite find_het_add_cet find_het_add_het_eq. done.
+    + move/negP: Heq => Hneq. 
+      rewrite (find_cet_add_cet_neq _ _ _ Hneq) find_cet_add_het => Hfcete2.
+      rewrite find_het_add_cet (find_het_add_het_neq _ _ _ Hneq). 
+      exact: (well_formed_find_cet Hwfc Hfcete2).
+  - move=> e2 cs2 l2. rewrite find_cbt_add_cet find_cbt_add_het.
+    rewrite find_hbt_add_cet find_hbt_add_het.
+    move=> Hfcbte2. exact: (well_formed_find_cbt Hwfc Hfcbte2).
+Qed.
 
 Lemma well_formed_add_cbt_hbt :
   forall c e cs l,
     well_formed c -> well_formed (add_cbt e cs l (add_hbt e cs l c)).
-Proof. Admitted.
+Proof.
+  move=> c e1 cs1 l1 Hwfc. split.
+  - move=> e2 cs2 ls2. rewrite find_cet_add_cbt find_cet_add_hbt.
+    rewrite find_het_add_cbt find_het_add_hbt.
+    move=> Hfcete2. exact: (well_formed_find_cet Hwfc Hfcete2).
+  - move=> e2 cs2 l2. case Heq : (e2 == e1).
+    + move/eqP: Heq => ->. rewrite find_cbt_add_cbt_eq. case=> <- <-.
+      rewrite find_hbt_add_cbt find_hbt_add_hbt_eq. done.
+    + move/negP: Heq => Hneq. 
+      rewrite (find_cbt_add_cbt_neq _ _ _ Hneq) find_cbt_add_hbt => Hfcbte2.
+      rewrite find_hbt_add_cbt (find_hbt_add_hbt_neq _ _ _ Hneq). 
+      exact: (well_formed_find_cbt Hwfc Hfcbte2).
+Qed.
 
-Lemma reset_ct_well_formed :
+Lemma well_formed_reset_ct :
   forall c, well_formed (reset_ct c).
 Proof.
-(*   done. *)
-(* Qed. *)
-Admitted.
+  done. 
+Qed.
 
 
 (* ==== interp_cache === *)
 
-Definition interp_cache_ct (E : env) (c : compcache) := CompTable.interp_table E (ct c).
-Definition interp_cache_ht (E : env) (c : compcache) := CompTable.interp_table E (ht c).
+Definition interp_cache_ct (E : env) (c : compcache) := 
+  CompTable.interp_table E (ct c).
+
+Definition interp_cache_ht (E : env) (c : compcache) := 
+  CompTable.interp_table E (ht c).
+
 Definition interp_cache := interp_cache_ht.
+
+Lemma interp_cache_well_formed_interp_ct :
+  forall E c, interp_cache E c -> well_formed c -> interp_cache_ct E c.
+Proof.
+  move=> E c [Hie Hib] [Hwfe Hwfb]. split.
+  - move=> e cs ls Hfind. move: (Hwfe _ _ _ Hfind). exact: Hie.
+  - move=> e cs l Hfind. move: (Hwfb _ _ _ Hfind). exact: Hib.
+Qed.
 
 Lemma interp_cache_ct_find_cet :
   forall E c e cs ls,
     interp_cache_ct E c -> find_cet e c = Some (cs, ls) -> interp_cnf E cs.
 Proof.
-Admitted.
+  move=> E c e cs ls. exact: CompTable.interp_table_find_et.
+Qed.
 
 Lemma interp_cache_ct_find_cbt :
   forall E c e cs l,
     interp_cache_ct E c -> find_cbt e c = Some (cs, l) -> interp_cnf E cs.
 Proof.
-Admitted.
+  move=> E c e cs l. exact: CompTable.interp_table_find_bt.
+Qed.
 
 Lemma interp_cache_find_het :
   forall E c e cs ls,
     interp_cache E c -> find_het e c = Some (cs, ls) -> interp_cnf E cs.
 Proof.
-Admitted.
+  move=> E c e cs ls. exact: CompTable.interp_table_find_et.
+Qed.
 
 Lemma interp_cache_find_hbt :
   forall E c e cs l,
     interp_cache E c -> find_hbt e c = Some (cs, l) -> interp_cnf E cs.
 Proof.
-Admitted.
+  move=> E c e cs l. exact: CompTable.interp_table_find_bt.
+Qed.
 
+Lemma interp_cache_ct_add_het :
+  forall E c e cs ls, interp_cache_ct E c <-> interp_cache_ct E (add_het e cs ls c).
+Proof. 
+  done.
+Qed.
+
+Lemma interp_cache_ct_add_hbt :
+  forall E c e cs l, interp_cache_ct E c <-> interp_cache_ct E (add_hbt e cs l c).
+Proof. 
+  done. 
+Qed.
+
+Lemma interp_cache_ct_add_cet :
+  forall E c e cs ls, interp_cache_ct E c -> interp_cnf E cs ->
+                      interp_cache_ct E (add_cet e cs ls c).
+Proof. 
+  move=> E c e cs ls. rewrite /interp_cache_ct /=. 
+  exact: CompTable.interp_table_add_et.
+Qed.
+
+Lemma interp_cache_ct_add_cbt :
+  forall E c e cs l, interp_cache_ct E c -> interp_cnf E cs ->
+                     interp_cache_ct E (add_cbt e cs l c).
+Proof. 
+  move=> E c e cs l. rewrite /interp_cache_ct /=. 
+  exact: CompTable.interp_table_add_bt.
+Qed.
+
+Lemma interp_cache_ct_reset_ct :
+  forall E c, interp_cache_ct E (reset_ct c).
+Proof.
+  done.
+Qed.
+
+Lemma interp_cache_add_het :
+  forall E c e cs ls, interp_cache E c -> interp_cnf E cs ->
+                      interp_cache E (add_het e cs ls c).
+Proof.
+  move=> E c e cs ls. rewrite /interp_cache /interp_cache_ht /=. 
+  exact: CompTable.interp_table_add_et.
+Qed.
+
+Lemma interp_cache_add_hbt :
+  forall E c e cs l, interp_cache E c -> interp_cnf E cs ->
+                     interp_cache E (add_hbt e cs l c).
+Proof.
+  move=> E c e cs l. rewrite /interp_cache /interp_cache_ht /=. 
+  exact: CompTable.interp_table_add_bt.
+Qed.
 
 Lemma interp_cache_add_cet :
   forall E c e cs ls, interp_cache E c <-> interp_cache E (add_cet e cs ls c).
@@ -306,154 +411,58 @@ Proof.
   move=> E c e cs ls. by rewrite /interp_cache. 
 Qed.
 
-Lemma interp_cache_add_het :
-  forall E c e cs ls, interp_cache E c -> interp_cnf E cs ->
-                      interp_cache E (add_het e cs ls c).
-Proof.
-(*   move=> E c e cs ls. rewrite /interp_cache /interp_cache_ht /add_het /=.  *)
-(*   by apply: CompTable.interp_table_add_et. *)
-(* Qed. *)
-Admitted.
-
-Lemma interp_cache_add_hbt :
-  forall E c e cs l, interp_cache E c -> interp_cnf E cs ->
-                     interp_cache E (add_hbt e cs l c).
-Proof.
-(*   move=> E c e cs l. rewrite /interp_cache /interp_cache_ht /add_hbt /=.  *)
-(*   by apply: CompTable.interp_table_add_bt. *)
-(* Qed. *)
-Admitted.
-
 Lemma interp_cache_reset_ct :
   forall E c, interp_cache E c <-> interp_cache E (reset_ct c).
-Proof.
-(*   move=> E c. by rewrite /interp_cache. *)
-(* Qed. *)
-Admitted.
+Proof. 
+  done.
+Qed.
 
-Lemma interp_cache_ct_add_cet :
-  forall E c e cs ls, interp_cache_ct E c -> interp_cnf E cs ->
-                      interp_cache_ct E (add_cet e cs ls c).
-Proof. Admitted.
-
-Lemma interp_cache_ct_add_cbt :
-  forall E c e cs l, interp_cache_ct E c -> interp_cnf E cs ->
-                     interp_cache_ct E (add_cbt e cs l c).
-Proof. Admitted.
-
-Lemma interp_cache_ct_add_het :
-  forall E c e cs ls, interp_cache_ct E c <-> interp_cache_ct E (add_het e cs ls c).
-Proof. Admitted.
-
-Lemma interp_cache_ct_add_hbt :
-  forall E c e cs l, interp_cache_ct E c <-> interp_cache_ct E (add_hbt e cs l c).
-Proof. Admitted.
-
-
-Lemma interp_cache_ct_reset_ct :
-  forall E c, interp_cache_ct E (reset_ct c).
-Proof.
-Admitted.
 
 (* ==== correct ==== *)
 
 Definition ht_enc_correct_exp e cs ls vm c := 
   CompTable.enc_correct_exp e cs ls vm (ht c).
+
 Definition ht_enc_correct_bexp e cs l vm c := 
   CompTable.enc_correct_bexp e cs l vm (ht c).
+
 Definition ct_enc_correct_exp e cs ls vm c := 
   CompTable.enc_correct_exp e cs ls vm (ct c).
+
 Definition ct_enc_correct_bexp e cs l vm c := 
   CompTable.enc_correct_bexp e cs l vm (ct c).
 
-(* Definition correct_ht (vm : vm) (c : compcache) := CompTable.correct vm (ht c). *)
-(* Definition correct_ct (vm : vm) (c : compcache) := CompTable.correct vm (ct c). *)
-Definition correct_ht (vm : vm) (c : compcache) :=
-  (forall e cs ls, find_het e c = Some (cs, ls) -> ht_enc_correct_exp e cs ls vm c)
-  /\ forall e cs l, find_hbt e c = Some (cs, l) -> ht_enc_correct_bexp e cs l vm c.
-Definition correct_ct (vm : vm) (c : compcache) :=
-  (forall e cs ls, find_cet e c = Some (cs, ls) -> ct_enc_correct_exp e cs ls vm c)
-  /\ forall e cs l, find_cbt e c = Some (cs, l) -> ct_enc_correct_bexp e cs l vm c.
+Definition correct_ht (vm : vm) (c : compcache) := CompTable.correct vm (ht c).
+Definition correct_ct (vm : vm) (c : compcache) := CompTable.correct vm (ct c).
 Definition correct (vm : vm) (c : compcache) := correct_ht vm c /\ correct_ct vm c.
-
-(*
-Lemma add_het_find_none_enc_correct_exp :
-  forall e c e0 cs0 ls0 vm cs ls,
-    find_het e c = None ->
-    ht_enc_correct_exp e0 cs0 ls0 vm c ->
-    ht_enc_correct_exp e0 cs0 ls0 vm (add_het e cs ls c).
-Proof.
-  move=> e cc e0 cs0 ls0 vm cs ls Hfe.
-  case e0 => /=.
-  - done.
-  - done.
-  - move=> op e1 [cs1 [ls1 [Hfe1 Hence]]].
-    exists cs1, ls1. split; last done.
-    rewrite -Hfe1. apply find_het_add_het_neq. by auto_prove_neq.
-  - move=> op e1 e2 [cs1 [ls1 [cs2 [ls2 [Hfe1 [Hfe2 Hence]]]]]].
-    exists cs1, ls1, cs2, ls2.     
-    split; last split; last done; [rewrite -Hfe1 | rewrite -Hfe2]; 
-      apply find_het_add_het_neq; by auto_prove_neq.
-  - move=> c e1 e2 [csc [lc [cs1 [ls1 [cs2 [ls2 [Hfc [Hfe1 [Hfe2 Hence]]]]]]]]].
-    exists csc, lc, cs1, ls1, cs2, ls2.
-    repeat split; last done.
-    + rewrite -Hfc. by apply find_hbt_add_het. 
-    + rewrite -Hfe1. apply find_het_add_het_neq. by auto_prove_neq.
-    + rewrite -Hfe2. apply find_het_add_het_neq. by auto_prove_neq.
-Qed.
-
-Lemma add_het_find_none_enc_correct_bexp :
-  forall e c e0 cs0 l0 vm cs ls,
-    find_het e c = None ->
-    ht_enc_correct_bexp e0 cs0 l0 vm c ->
-    ht_enc_correct_bexp e0 cs0 l0 vm (add_het e cs ls c).
-Proof.
-  move=> e cc e0 cs0 l0 vm cs ls Hfe.
-  case e0 => /=.
-  - done.
-  - done.
-  - move=> op e1 e2 [cs1 [ls1 [cs2 [ls2 [Hfe1 [Hfe2 Hence]]]]]].
-    exists cs1, ls1, cs2, ls2.     
-    split; last split; last done; [rewrite -Hfe1 | rewrite -Hfe2];
-      apply find_het_add_het_neq; by auto_prove_neq.
-  - move=> e1 [cs1 [l1 [Hfe1 Hence]]].
-    exists cs1, l1. split; last done.
-    rewrite -Hfe1. by apply find_hbt_add_het. 
-  - move=> e1 e2 [cs1 [l1 [cs2 [l2 [Hfe1 [Hfe2 Hence]]]]]].
-    exists cs1, l1, cs2, l2.     
-    split; last split; last done; [rewrite -Hfe1 | rewrite -Hfe2];
-      by apply find_hbt_add_het.
-  - move=> e1 e2 [cs1 [l1 [cs2 [l2 [Hfe1 [Hfe2 Hence]]]]]].
-    exists cs1, l1, cs2, l2.     
-    split; last split; last done; [rewrite -Hfe1 | rewrite -Hfe2];
-      by apply find_hbt_add_het.
-Qed.
-*)
-
-Lemma correct_find_cet :
-  forall m c e cs ls,
-  correct m c -> find_cet e c = Some (cs, ls) -> ct_enc_correct_exp e cs ls m c.
-Proof.
-Admitted.
 
 Lemma correct_find_het :
   forall m c e cs ls,
   correct m c -> find_het e c = Some (cs, ls) -> ht_enc_correct_exp e cs ls m c.
 Proof.
-Admitted.
-
-Lemma correct_find_cbt :
-  forall m c e cs l,
-  correct m c -> find_cbt e c = Some (cs, l) -> ct_enc_correct_bexp e cs l m c.
-Proof.
-Admitted.
+  move=> m c e cs ls [Hcrht Hcrct]. exact: CompTable.correct_find_et.
+Qed.
 
 Lemma correct_find_hbt :
   forall m c e cs l,
   correct m c -> find_hbt e c = Some (cs, l) -> ht_enc_correct_bexp e cs l m c.
 Proof.
-Admitted.
+  move=> m c e cs l [Hcrht Hcrct]. exact: CompTable.correct_find_bt.
+Qed.
 
+Lemma correct_find_cet :
+  forall m c e cs ls,
+  correct m c -> find_cet e c = Some (cs, ls) -> ct_enc_correct_exp e cs ls m c.
+Proof.
+  move=> m c e cs ls [Hcrht Hcrct]. exact: CompTable.correct_find_et.
+Qed.
+
+Lemma correct_find_cbt :
+  forall m c e cs l,
+  correct m c -> find_cbt e c = Some (cs, l) -> ct_enc_correct_bexp e cs l m c.
+Proof.
+  move=> m c e cs l [Hcrht Hcrct]. exact: CompTable.correct_find_bt.
+Qed.
 
 Lemma correct_ht_add_het :
   forall vm c e cs ls, 
@@ -464,6 +473,41 @@ Lemma correct_ht_add_het :
 Proof.
   move=> vm c e cs ls. rewrite /correct_ht /find_het /ht_enc_correct_exp /=.
   by apply: CompTable.correct_add_et.
+Qed.
+
+Lemma correct_ht_add_hbt :
+  forall vm c e cs l, 
+    correct_ht vm c
+    -> find_hbt e c = None
+    -> ht_enc_correct_bexp e cs l vm c
+    -> correct_ht vm (add_hbt e cs l c).
+Proof.
+  move=> vm c e cs l. rewrite /correct_ht /find_hbt /ht_enc_correct_bexp /=.
+  by apply: CompTable.correct_add_bt.
+Qed.
+
+Lemma correct_ht_add_cet :
+  forall vm c e cs ls, correct_ht vm c <-> correct_ht vm (add_cet e cs ls c).
+Proof.
+  move=> vm c e cs ls. rewrite /correct_ht. done. 
+Qed.
+
+Lemma correct_ht_add_cbt :
+  forall vm c e cs l, correct_ht vm c <-> correct_ht vm (add_cbt e cs l c).
+Proof.
+  move=> vm c e cs l. rewrite /correct_ht. done. 
+Qed.
+
+Lemma correct_ct_add_het :
+  forall vm c e cs ls, correct_ct vm c <-> correct_ct vm (add_het e cs ls c).
+Proof.
+  move=> vm c e cs ls. rewrite /correct_ct. done. 
+Qed.
+
+Lemma correct_ct_add_hbt :
+  forall vm c e cs l, correct_ct vm c <-> correct_ct vm (add_hbt e cs l c).
+Proof.
+  move=> vm c e cs l. rewrite /correct_ct. done. 
 Qed.
 
 Lemma correct_ct_add_cet :
@@ -477,6 +521,17 @@ Proof.
   by apply: CompTable.correct_add_et.
 Qed.
 
+Lemma correct_ct_add_cbt :
+  forall vm c e cs l, 
+    correct_ct vm c
+    -> find_cbt e c = None
+    -> ct_enc_correct_bexp e cs l vm c
+    -> correct_ct vm (add_cbt e cs l c).
+Proof.
+  move=> vm c e cs l. rewrite /correct_ct /find_cbt /ct_enc_correct_bexp /=.
+  by apply: CompTable.correct_add_bt.
+Qed.
+
 Lemma correct_add_cet :
   forall vm c e cs ls, 
     correct vm c
@@ -484,9 +539,10 @@ Lemma correct_add_cet :
     -> ct_enc_correct_exp e cs ls vm c
     -> correct vm (add_cet e cs ls c).
 Proof.
-  (* move=> vm c e cs ls. rewrite /correct_ct /find_cet /ct_enc_correct_exp /=. *)
-  (* by apply: CompTable.correct_add_et. *)
-Admitted.
+  move=> vm c e cs ls [Hctc Hhtc] Hfcet Hctenc. split.
+  - rewrite -correct_ht_add_cet. done.
+  - by apply correct_ct_add_cet.
+Qed.
 
 Lemma correct_add_cet_het :
   forall vm c e cs ls, 
@@ -497,9 +553,10 @@ Lemma correct_add_cet_het :
     -> ht_enc_correct_exp e cs ls vm c
     -> correct vm (add_cet e cs ls (add_het e cs ls c)).
 Proof.
-  (* move=> vm c e cs ls. rewrite /correct_ct /find_cet /ct_enc_correct_exp /=. *)
-  (* by apply: CompTable.correct_add_et. *)
-Admitted.
+  move=> vm c e cs ls [Hctc Hhtc] Hfcet Hfhet Hctenc Hhtenc. split. 
+  - rewrite -correct_ht_add_cet. by apply correct_ht_add_het.
+  - rewrite -add_het_cet_comm -correct_ct_add_het. by apply correct_ct_add_cet. 
+Qed.
 
 Lemma correct_add_cbt :
   forall vm c e cs l, 
@@ -508,9 +565,10 @@ Lemma correct_add_cbt :
     -> ct_enc_correct_bexp e cs l vm c
     -> correct vm (add_cbt e cs l c).
 Proof.
-  (* move=> vm c e cs ls. rewrite /correct_ct /find_cet /ct_enc_correct_exp /=. *)
-  (* by apply: CompTable.correct_add_et. *)
-Admitted.
+  move=> vm c e cs l [Hctc Hhtc] Hfcbt Hctenc. split.
+  - rewrite -correct_ht_add_cbt. done.
+  - by apply correct_ct_add_cbt.
+Qed.
 
 Lemma correct_add_cbt_hbt :
   forall vm c e cs l, 
@@ -521,180 +579,45 @@ Lemma correct_add_cbt_hbt :
     -> ht_enc_correct_bexp e cs l vm c
     -> correct vm (add_cbt e cs l (add_hbt e cs l c)).
 Proof.
-  (* move=> vm c e cs ls. rewrite /correct_ct /find_cet /ct_enc_correct_exp /=. *)
-  (* by apply: CompTable.correct_add_et. *)
-Admitted.
+  move=> vm c e cs l [Hctc Hhtc] Hfcbt Hfhbt Hctenc Hhtenc. split. 
+  - rewrite -correct_ht_add_cbt. by apply correct_ht_add_hbt.
+  - rewrite -add_hbt_cbt_comm -correct_ct_add_hbt. by apply correct_ct_add_cbt. 
+Qed.
 
 Lemma correct_reset_ct :
   forall vm c, correct vm c -> correct vm (reset_ct c).
 Proof.
-Admitted.
-
-
-(*
-Lemma correct_add_cbt :
-  forall vm c e cs l, correct vm c <-> correct vm (add_cbt e cs l c).
-Proof.
-  move=> vm c e cs l. done.
+  move=> vm c [Hct Hht]. split; done.
 Qed.
-
-Lemma correct_add_het :
-  forall vm c e cs ls, 
-    correct vm c -> (forall vm, consistent vm vm -> enc_correct_exp e cs ls vm c)
-    -> correct vm (add_het e cs ls c).
-Proof.
-  move=> vm c e cs ls [[Hce Hcb] Hence]. rewrite /strong_correct /=. 
-  split; last done.
-  move=> e0 cs0 ls0. case Heq : (e0 == e).
-  - rewrite (ExpMap.Lemmas.find_add_eq Heq). move/eqP: Heq => Heq.
-    rewrite Heq. case=> <- <-; done.
-  - move/negP: Heq => Heq. rewrite (ExpMap.Lemmas.find_add_neq Heq).
-    exact: Hce.
-Qed.
-*)
-
-(*
-Lemma strong_correct_add_hbt :
-  forall vm c e cs l, strong_correct vm c /\ enc_correct_bexp vm e cs l ->
-                      strong_correct vm (add_hbt e cs l c).
-Proof.
-  move=> vm c e cs l [[Hce Hcb] Hence]. rewrite /strong_correct /=.
-  split; first done.
-  move=> e0 cs0 l0. case Heq : (e0 == e).
-  - rewrite (BexpMap.Lemmas.find_add_eq Heq). move/eqP: Heq => Heq.
-    rewrite Heq. case=> <- <-; done.
-  - move/negP: Heq => Heq. rewrite (BexpMap.Lemmas.find_add_neq Heq).
-    exact: Hcb.
-Qed.
-
-Lemma strong_correct_reset_ct :
-  forall vm c, strong_correct vm c <-> strong_correct vm (reset_ct c).
-Proof.
-  move=> vm c. done. 
-Qed.
-
-
-
-Lemma correct_add_cet :
-  forall vm c e ls, correct vm c <-> correct vm (add_cet e ls c).
-Proof.
-  move=> vm c e ls. by rewrite /correct. 
-Qed.
-
-Lemma correct_add_cbt :
-  forall vm c e l, correct vm c <-> correct vm (add_cbt e l c).
-Proof.
-  move=> E c e ls. by rewrite /correct. 
-Qed.
-
-Lemma correct_add_het :
-  forall vm c e cs ls, correct vm c /\ enc_bits E ls (QFBV.eval_exp e s) ->
-                        correct vm (add_het e cs ls c).
-Proof.
-  move=> vm c e cs ls [[Hce Hcb] Hence]. rewrite /correct /=. split; last done.
-  move=> e0 cs0 ls0. case Heq : (e0 == e).
-  - rewrite (ExpMap.Lemmas.find_add_eq Heq). move/eqP: Heq => Heq.
-    rewrite Heq. case=> _ <-; done.
-  - move/negP: Heq => Heq. rewrite (ExpMap.Lemmas.find_add_neq Heq).
-    exact: Hce.
-Qed.
-
-Lemma correct_add_hbt :
-  forall vm c e cs l, correct vm c /\ enc_bit E l (QFBV.eval_bexp e s) ->
-                       correct vm (add_hbt e cs l c).
-Proof.
-  move=> vm c e cs l [[Hce Hcb] Hence]. rewrite /correct /=. split; first done.
-  move=> e0 cs0 l0. case Heq : (e0 == e).
-  - rewrite (BexpMap.Lemmas.find_add_eq Heq). move/eqP: Heq => Heq.
-    rewrite Heq. case=> _ <-; done.
-  - move/negP: Heq => Heq. rewrite (BexpMap.Lemmas.find_add_neq Heq).
-    exact: Hcb.
-Qed.
-*)
-
-(*
-Lemma correct_reset_ct :
-  forall vm c, correct vm c <-> correct vm (reset_ct c).
-Proof.
-  move=> vm c. by rewrite /correct.
-Qed.
-*)
-
-
-
-(*
-Lemma vm_preserve_enc_correct_exp :
-  forall m m' e cs ls, 
-    vm_preserve m m' -> enc_correct_exp m e cs ls -> enc_correct_exp m' e cs ls.
-Proof.
-  move=> m m' e cs ls Hpmmp. rewrite /enc_correct_exp.
-  move=> Henc vm Hconmp Hics.
-  move: (vm_preserve_consistent Hpmmp Hconmp) => Hconm.
-  by apply: Henc.
-Qed.
-
-Lemma vm_preserve_enc_correct_bexp :
-  forall m m' e cs l, 
-    vm_preserve m m' -> enc_correct_bexp m e cs l -> enc_correct_bexp m' e cs l.
-Proof.
-  move=> m m' e cs l Hpmmp. rewrite /enc_correct_bexp.
-  move=> Henc vm Hconmp Hics.
-  move: (vm_preserve_consistent Hpmmp Hconmp) => Hconm.
-  by apply: Henc.
-Qed.
-
-Lemma vm_preserve_strong_correct :
-  forall m m' c, vm_preserve m m' -> strong_correct m c -> strong_correct m' c.
-Proof.
-  move=> m m' c Hpmmp [Hce Hcb]. rewrite /strong_correct. split.
-  - move=> e cs ls Hfind. move: (Hce _ _ _ Hfind) => Hencm.
-    by apply: (@vm_preserve_enc_correct_exp m).
-  - move=> e cs l Hfind. move: (Hcb _ _ _ Hfind) => Hencm.
-    by apply: (@vm_preserve_enc_correct_bexp m).
-Qed.
-*)
 
 Lemma vm_preserve_correct :
   forall m m' c, vm_preserve m m' -> correct m c -> correct m' c.
 Proof.
-(*   move=> m m' c Hpmmp [Hce Hcb]. rewrite /correct. split. *)
-(*   - move=> e cs ls Hfind. move: (Hce _ _ _ Hfind) => Hencm. *)
-(*     by apply: (@vm_preserve_enc_correct_exp m). *)
-(*   - move=> e cs l Hfind. move: (Hcb _ _ _ Hfind) => Hencm. *)
-(*     by apply: (@vm_preserve_enc_correct_bexp m). *)
-(* Qed. *)
-Admitted.
-
+  move=> m m' c Hpre [Hht Hct]. 
+  split; by apply (@CompTable.vm_preserve_correct m).
+Qed.
 
 Lemma interp_cache_ct_find_cet_some_correct :
   forall m E s c e cs ls,
     consistent m E s -> interp_lit E lit_tt
     -> interp_cache_ct E c -> find_cet e c = Some (cs, ls) 
-    -> correct m c -> enc_bits E ls (QFBV.eval_exp e s)
-  with
-    interp_cache_ct_find_cbt_some_correct :
-      forall m E s c e cs l,
-        consistent m E s -> interp_lit E lit_tt
-        -> interp_cache_ct E c -> find_cbt e c = Some (cs, l) 
-        -> correct m c -> enc_bit E l (QFBV.eval_bexp e s).
+    -> correct m c -> enc_bits E ls (QFBV.eval_exp e s).
 Proof.
-  (* interp_cache_ct_find_cet_some_correct *)
-  move=> m E s c.
-  elim => [v | bs | op e1 IH1 | op e1 IH1 e2 IH2 | b e1 IH1 e2 IH2];
-  move=> cs ls Hcon Htt HrEc Hfe Hcrmc;
-  move: (interp_cache_ct_find_cet HrEc Hfe) => Hics;
-  move: (add_prelude_to Htt Hics) => {Hics} Hics.
-  - move: (correct_find_cet Hcrmc Hfe) => /= Hence.
-    by apply Hence.
-  - admit.
-  - admit.
-  - move: (correct_find_cet Hcrmc Hfe) => /= 
-      [cs1 [ls1 [cs2 [ls2 [Hfe1 [Hfe2 Hence]]]]]].
-    rewrite /find_cet in IH1 IH2.
-    move: (IH1 _ _ Hcon Htt HrEc Hfe1 Hcrmc) 
-            (IH2 _ _ Hcon Htt HrEc Hfe2 Hcrmc) => Henc1 Henc2.
-    by apply Hence.
-Admitted.
+  move=> m E s c e cs ls Hcon Htt HiEc Hfe [Hcrht Hcrct].
+  move: HiEc Hfe Hcrct.
+  by apply CompTable.interp_table_find_et_some_correct.
+Qed.
+
+Lemma interp_cache_ct_find_cbt_some_correct :
+  forall m E s c e cs l,
+    consistent m E s -> interp_lit E lit_tt
+    -> interp_cache_ct E c -> find_cbt e c = Some (cs, l) 
+    -> correct m c -> enc_bit E l (QFBV.eval_bexp e s).
+Proof.
+  move=> m E s c e cs l Hcon Htt HiEc Hfe [Hcrht Hcrct].
+  move: HiEc Hfe Hcrct.
+  by apply CompTable.interp_table_find_bt_some_correct.
+Qed.
 
 
 (* ==== newer_than_cache ==== *)
@@ -706,67 +629,84 @@ Definition newer_than_cache := newer_than_ht.
 Lemma newer_than_cache_well_formed_newer_ct :
   forall g c, newer_than_cache g c -> well_formed c -> newer_than_ct g c.
 Proof.
-Admitted.
+  move=> g c [Hnewe Hnewb] [Hwfe Hwfb]. split.
+  - move=> e cs ls Hfcet. move: (Hwfe _ _ _ Hfcet). exact: Hnewe.
+  - move=> e cs l Hfcbt. move: (Hwfb _ _ _ Hfcbt). exact: Hnewb.
+Qed.
 
 Lemma newer_than_ct_find_cet :
   forall g c e cs ls,
     newer_than_ct g c -> find_cet e c = Some (cs, ls) 
     -> newer_than_cnf g cs /\ newer_than_lits g ls.
-Proof. Admitted.
+Proof.
+  move=> g c e cs ls. exact: CompTable.newer_than_table_find_et.
+Qed.
 
 Lemma newer_than_ct_find_cbt :
   forall g c e cs l,
     newer_than_ct g c -> find_cbt e c = Some (cs, l) 
     -> newer_than_cnf g cs /\ newer_than_lit g l.
-Proof. Admitted.
+Proof. 
+  move=> g c e cs l. exact: CompTable.newer_than_table_find_bt.
+Qed.
 
 Lemma newer_than_cache_find_het :
   forall g c e cs ls,
     newer_than_cache g c -> find_het e c = Some (cs, ls) 
     -> newer_than_cnf g cs /\ newer_than_lits g ls.
-Proof. Admitted.
+Proof.
+  move=> g c e cs ls. exact: CompTable.newer_than_table_find_et.
+Qed.
 
 Lemma newer_than_cache_find_hbt :
   forall g c e cs l,
     newer_than_cache g c -> find_hbt e c = Some (cs, l) 
     -> newer_than_cnf g cs /\ newer_than_lit g l.
-Proof. Admitted.
-
-
-Lemma newer_than_cache_add_cet :
-  forall g c e cs ls, 
-    newer_than_cache g c <-> newer_than_cache g (add_cet e cs ls c).
-Proof. Admitted.
-
-Lemma newer_than_cache_add_cbt :
-  forall g c e cs l, 
-    newer_than_cache g c <-> newer_than_cache g (add_cbt e cs l c).
-Proof. Admitted.
+Proof.
+  move=> g c e cs l. exact: CompTable.newer_than_table_find_bt.
+Qed.
 
 Lemma newer_than_cache_add_het :
   forall g c e cs ls, 
     newer_than_cache g c -> newer_than_cnf g cs -> newer_than_lits g ls 
     -> newer_than_cache g (add_het e cs ls c).
-Proof. Admitted.
+Proof. 
+  move=> g c e cs ls. exact: CompTable.newer_than_table_add_et.
+Qed.
 
 Lemma newer_than_cache_add_hbt :
   forall g c e cs l, 
     newer_than_cache g c -> newer_than_cnf g cs -> newer_than_lit g l 
     -> newer_than_cache g (add_hbt e cs l c).
-Proof. Admitted.
+Proof.
+  move=> g c e cs l. exact: CompTable.newer_than_table_add_bt.
+Qed.
 
+Lemma newer_than_cache_add_cet :
+  forall g c e cs ls, 
+    newer_than_cache g c <-> newer_than_cache g (add_cet e cs ls c).
+Proof.
+  done.
+Qed.
 
-Lemma newer_than_cache_le_newer g g' c :
-  newer_than_cache g c -> (g <=? g')%positive -> newer_than_cache g' c.
-Proof. Admitted.
-
+Lemma newer_than_cache_add_cbt :
+  forall g c e cs l, 
+    newer_than_cache g c <-> newer_than_cache g (add_cbt e cs l c).
+Proof.
+  done.
+Qed.
 
 Lemma newer_than_cache_reset_ct :
   forall g c, newer_than_cache g c <-> newer_than_cache g (reset_ct c).
-Proof.
-  move=> g c. by rewrite /newer_than_cache.
+Proof. 
+  done.
 Qed.
 
+Lemma newer_than_cache_le_newer g g' c :
+  newer_than_cache g c -> (g <=? g')%positive -> newer_than_cache g' c.
+Proof. 
+  exact: CompTable.newer_than_table_le_newer.
+Qed.
 
 Lemma env_preserve_interp_cache : 
   forall E E' g c,
@@ -777,26 +717,6 @@ Proof.
   by apply: CompTable.env_preserve_interp_table.
 Qed.    
 
-(*
-Lemma env_preserve_correct E E' s g ca :
-  env_preserve E E' g -> newer_than_cache g ca ->
-  correct E' s ca <-> correct vm ca.
-Proof.
-  move=> Henv [Hge Hgb]. rewrite /correct. split.
-  - apply env_preserve_sym in Henv. move=> [H1 H2]. 
-    split; move=> e cs ls Hfind.
-    + move: (Hge _ _ _ Hfind) => /andP [_ Hgls].
-      apply (env_preserve_enc_bits Henv Hgls). exact: (H1 _ _ _ Hfind).
-    + move: (Hgb _ _ _ Hfind) => /andP [_ Hgls].
-      apply (env_preserve_enc_bit Henv Hgls). exact: (H2 _ _ _ Hfind).
-  - move=> [H1 H2]. 
-    split; move=> e cs ls Hfind.
-    + move: (Hge _ _ _ Hfind) => /andP [_ Hgls].
-      apply (env_preserve_enc_bits Henv Hgls). exact: (H1 _ _ _ Hfind).
-    + move: (Hgb _ _ _ Hfind) => /andP [_ Hgls].
-      apply (env_preserve_enc_bit Henv Hgls). exact: (H2 _ _ _ Hfind).
-Qed.    
-*)
 
 (* ==== bound by vm ==== *)
 
@@ -807,67 +727,74 @@ Definition bound := bound_ht.
 Lemma bound_well_formed_bound_ct :
   forall c vm, bound c vm -> well_formed c -> bound_ct c vm.
 Proof.
-Admitted.
+  move=> c vm [Hbde Hbdb] [Hwfe Hwfb]. split.
+  - move=> e cs ls Hfind. move: (Hwfe _ _ _ Hfind). exact: Hbde.
+  - move=> e cs l Hfind. move: (Hwfb _ _ _ Hfind). exact: Hbdb.
+Qed.
 
 Lemma bound_ct_find_cet :
   forall c m e cs ls, 
-    bound_ct c m -> find_cet e c = Some (cs, ls)  -> bound_exp e m.
-Proof. Admitted.
+    bound_ct c m -> find_cet e c = Some (cs, ls) -> bound_exp e m.
+Proof. 
+  move=> c m e cs ls. exact: CompTable.bound_find_et.
+Qed.
 
 Lemma bound_ct_find_cbt :
   forall c m e cs l, 
     bound_ct c m -> find_cbt e c = Some (cs, l) -> bound_bexp e m.
-Proof. Admitted.
+Proof.
+  move=> c m e cs l. exact: CompTable.bound_find_bt.
+Qed.
 
 Lemma bound_find_het :
   forall c m e cs ls, 
-    bound c m -> find_het e c = Some (cs, ls)  -> bound_exp e m.
-Proof. Admitted.
+    bound c m -> find_het e c = Some (cs, ls) -> bound_exp e m.
+Proof.
+  move=> c m e cs ls. exact: CompTable.bound_find_et.
+Qed.
 
 Lemma bound_find_hbt :
   forall c m e cs l, 
     bound c m -> find_hbt e c = Some (cs, l) -> bound_bexp e m.
-Proof. Admitted.
-
-
-Lemma bound_add_cet :
-  forall c vm e cs ls, bound c vm <-> bound (add_cet e cs ls c) vm.
-Proof.
-  move=> c vm e cs ls. by rewrite /bound. 
-Qed.
-
-Lemma bound_add_cbt :
-  forall c vm e cs l, bound c vm <-> bound (add_cbt e cs l c) vm.
-Proof.
-  move=> c vm e cs l. by rewrite /bound. 
+Proof.  
+  move=> c m e cs l. exact: CompTable.bound_find_bt.
 Qed.
 
 Lemma bound_add_het :
   forall c vm e cs ls, bound c vm -> bound_exp e vm -> bound (add_het e cs ls c) vm.
 Proof.
-(*   move=> c vm e cs ls. rewrite /bound /bound_ht /add_het /=.  *)
-(*   by apply: CompTable.bound_add_et. *)
-(* Qed. *)
-Admitted.
+  move=> c vm e cs ls. exact: CompTable.bound_add_et.
+Qed.
 
 Lemma bound_add_hbt :
   forall c vm e cs l, bound c vm -> bound_bexp e vm -> bound (add_hbt e cs l c) vm.
 Proof.
-(*   move=> c vm e cs l. rewrite /bound /bound_ht /add_hbt /=.  *)
-(*   by apply: CompTable.bound_add_bt. *)
-(* Qed. *)
-Admitted.
+  move=> c vm e cs l. exact: CompTable.bound_add_bt.
+Qed.
+
+Lemma bound_add_cet :
+  forall c vm e cs ls, bound c vm <-> bound (add_cet e cs ls c) vm.
+Proof.
+  done.
+Qed.
+
+Lemma bound_add_cbt :
+  forall c vm e cs l, bound c vm <-> bound (add_cbt e cs l c) vm.
+Proof.
+  done.
+Qed.
 
 Lemma bound_reset_ct :
   forall c vm, bound c vm <-> bound (reset_ct c) vm.
 Proof.
-(*   move=> c vm. by rewrite /bound. *)
-(* Qed. *)
-Admitted.
+  done.
+Qed.
 
 Lemma vm_preserve_bound :
   forall m m' c, vm_preserve m m' -> bound c m -> bound c m'.
-Proof. Admitted.
+Proof.
+  move=> m m' c. exact: CompTable.vm_preserve_bound.
+Qed.
 
 (* Lemma bound_add_find_none : *)
 (*   forall c vm v ls, *)
@@ -883,56 +810,79 @@ Proof. Admitted.
 Definition preserve (c c' : compcache) : Prop :=
   CompTable.preserve (ct c) (ct c') /\ CompTable.preserve (ht c) (ht c').
 
-Lemma preserve_find_cet :
-  forall c c' e cs ls,
-    preserve c c' -> 
-    find_cet e c = Some (cs, ls) -> find_cet e c' = Some (cs, ls).
+Lemma preserve_refl : forall c, preserve c c.
 Proof.
-Admitted.
+  done.
+Qed.
 
-Lemma preserve_find_cbt :
-  forall c c' e cs l,
-    preserve c c' -> 
-    find_cbt e c = Some (cs, l) -> find_cbt e c' = Some (cs, l).
-Proof.
-Admitted.
+Lemma preserve_trans :
+  forall c1 c2 c3, preserve c1 c2 -> preserve c2 c3 -> preserve c1 c3.
+Proof. 
+  move=> c1 c2 c3 [Hpct12 Hpht12] [Hpct23 Hpht23]. split. 
+  - by apply (CompTable.preserve_trans Hpct12).
+  - by apply (CompTable.preserve_trans Hpht12).
+Qed.
 
 Lemma preserve_find_het :
   forall c c' e cs ls,
     preserve c c' -> 
     find_het e c = Some (cs, ls) -> find_het e c' = Some (cs, ls).
 Proof.
-Admitted.
+  move=> c c' e cs ls [Hprect Hpreht]. exact: CompTable.preserve_find_et.
+Qed.
 
 Lemma preserve_find_hbt :
   forall c c' e cs l,
     preserve c c' -> 
     find_hbt e c = Some (cs, l) -> find_hbt e c' = Some (cs, l).
 Proof.
-Admitted.
+  move=> c c' e cs l [Hprect Hpreht]. exact: CompTable.preserve_find_bt.
+Qed.
 
-Lemma preserve_add_cet :
-  forall c1 c2 e cs ls,
-    preserve c1 c2 -> find_cet e c2 = None -> preserve c1 (add_cet e cs ls c2).
-Proof. Admitted.
+Lemma preserve_find_cet :
+  forall c c' e cs ls,
+    preserve c c' -> 
+    find_cet e c = Some (cs, ls) -> find_cet e c' = Some (cs, ls).
+Proof.
+  move=> c c' e cs ls [Hprect Hpreht]. exact: CompTable.preserve_find_et.
+Qed.
 
-Lemma preserve_add_cbt :
-  forall c1 c2 e cs l,
-    preserve c1 c2 -> find_cbt e c2 = None -> preserve c1 (add_cbt e cs l c2).
-Proof. Admitted.
+Lemma preserve_find_cbt :
+  forall c c' e cs l,
+    preserve c c' -> 
+    find_cbt e c = Some (cs, l) -> find_cbt e c' = Some (cs, l).
+Proof.
+  move=> c c' e cs l [Hprect Hpreht]. exact: CompTable.preserve_find_bt.
+Qed.
 
 Lemma preserve_add_het :
   forall c1 c2 e cs ls,
     preserve c1 c2 -> find_het e c2 = None -> preserve c1 (add_het e cs ls c2).
-Proof. Admitted.
+Proof. 
+  move=> c1 c2 e cs ls [Hpct Hpht] Hfe. 
+  split; rewrite /=; [ done | exact: CompTable.preserve_add_et ].
+Qed.
 
 Lemma preserve_add_hbt :
   forall c1 c2 e cs l,
     preserve c1 c2 -> find_hbt e c2 = None -> preserve c1 (add_hbt e cs l c2).
-Proof. Admitted.
+Proof.
+  move=> c1 c2 e cs l [Hpct Hpht] Hfe. 
+  split; rewrite /=; [ done | exact: CompTable.preserve_add_bt ].
+Qed.
 
-Lemma preserve_trans :
-  forall c1 c2 c3,
-    preserve c1 c2 -> preserve c2 c3 -> preserve c1 c3.
-Proof. Admitted.
+Lemma preserve_add_cet :
+  forall c1 c2 e cs ls,
+    preserve c1 c2 -> find_cet e c2 = None -> preserve c1 (add_cet e cs ls c2).
+Proof. 
+  move=> c1 c2 e cs ls [Hpct Hpht] Hfe. 
+  split; rewrite /=; [ exact: CompTable.preserve_add_et | done ].
+Qed.
 
+Lemma preserve_add_cbt :
+  forall c1 c2 e cs l,
+    preserve c1 c2 -> find_cbt e c2 = None -> preserve c1 (add_cbt e cs l c2).
+Proof.
+  move=> c1 c2 e cs l [Hpct Hpht] Hfe. 
+  split; rewrite /=; [ exact: CompTable.preserve_add_bt | done ].
+Qed.
