src/newBBCache/CompTable.v
@@ -7,24 +7,34 @@ Set Implicit Arguments.
 Unset Strict Implicit.
 Import Prenex Implicits.
 
+
 Module ExpMap <: SsrFMap := FMaps.MakeTreeMap QFBV.ExpOrder.
 Module BexpMap <: SsrFMap := FMaps.MakeTreeMap QFBV.BexpOrder.
 
 Definition expm := ExpMap.t (cnf * word).
 Definition bexpm := BexpMap.t (cnf * literal).
 
-(* ==== A table storing complete results, including CNF and literal(s) ==== *)
+
+(* == A table storing complete results, including CNF and literal(s) == *)
 
 Record comptable :=
   { et : expm;
     bt : bexpm }.
 
+Definition empty : comptable := 
+  {| et := ExpMap.empty (cnf * word);
+     bt := BexpMap.empty (cnf * literal) |}.
+
 Definition find_et e t := ExpMap.find e (et t).
 Definition find_bt e t := BexpMap.find e (bt t).
+
+
+(* ==== modification ==== *)
 
 Definition add_et e cs ls t := 
   {| et := ExpMap.add e (cs, ls) (et t);
      bt := bt t |}.
+
 Definition add_bt e cs l t := 
   {| et := et t;
      bt := BexpMap.add e (cs, l) (bt t) |}.
@@ -36,23 +46,10 @@ Proof.
   by apply: ExpMap.Lemmas.find_add_eq.
 Qed.
 
-Lemma find_bt_add_bt_eq :
-  forall e cs l t, find_bt e (add_bt e cs l t) = Some (cs, l).
-Proof.
-  move=> e cs l t. rewrite /find_bt /add_bt /=. 
-  by apply: BexpMap.Lemmas.find_add_eq.
-Qed.
-
 Lemma find_et_add_et_neq :
   forall e0 e cs ls t, ~ e0 == e -> find_et e0 (add_et e cs ls t) = find_et e0 t.
 Proof.
   move=> e0 e cs ls t Hneq. by apply: ExpMap.Lemmas.find_add_neq.
-Qed.
-
-Lemma find_bt_add_bt_neq :
-  forall e0 e cs l t, ~ e0 == e -> find_bt e0 (add_bt e cs l t) = find_bt e0 t .
-Proof.
-  move=> e0 e cs l t Hneq. by apply: BexpMap.Lemmas.find_add_neq. 
 Qed.
 
 Lemma find_et_add_bt :
@@ -67,6 +64,19 @@ Proof.
   move=> e0 e cs ls t. done. 
 Qed.
 
+Lemma find_bt_add_bt_eq :
+  forall e cs l t, find_bt e (add_bt e cs l t) = Some (cs, l).
+Proof.
+  move=> e cs l t. rewrite /find_bt /add_bt /=. 
+  by apply: BexpMap.Lemmas.find_add_eq.
+Qed.
+
+Lemma find_bt_add_bt_neq :
+  forall e0 e cs l t, ~ e0 == e -> find_bt e0 (add_bt e cs l t) = find_bt e0 t .
+Proof.
+  move=> e0 e cs l t Hneq. by apply: BexpMap.Lemmas.find_add_neq. 
+Qed.
+
 
 (* ==== interp_table === *)
 
@@ -74,11 +84,25 @@ Definition interp_table (E : env) (t : comptable) :=
   (forall e cs ls, find_et e t = Some (cs, ls) -> interp_cnf E cs)
   /\ forall e cs l, find_bt e t = Some (cs, l) -> interp_cnf E cs.
 
+Lemma interp_table_find_et :
+  forall E t e cs ls,
+    interp_table E t -> find_et e t = Some (cs, ls) -> interp_cnf E cs.
+Proof.
+  move=> E t e cs ls [Hie Hib]. by apply Hie.
+Qed.
+
+Lemma interp_table_find_bt :
+  forall E t e cs l,
+    interp_table E t -> find_bt e t = Some (cs, l) -> interp_cnf E cs.
+Proof.
+  move=> E t e cs l [Hie Hib]. by apply Hib.
+Qed.
+
 Lemma interp_table_add_et :
-  forall E t e cs ls, interp_table E t /\ interp_cnf E cs ->
+  forall E t e cs ls, interp_table E t -> interp_cnf E cs ->
                       interp_table E (add_et e cs ls t).
 Proof.
-  move=> E t e cs ls [[Hre Hrb] Hcs]. rewrite /interp_table /=. split; last done.
+  move=> E t e cs ls [Hre Hrb] Hcs. rewrite /interp_table /=. split; last done.
   move=> e0 cs0 ls0. case Heq : (e0 == e).
   - move/eqP: Heq => <-. rewrite find_et_add_et_eq. case=> <- _; done.
   - move/negP: Heq => Hneq. rewrite (find_et_add_et_neq _ _ _ Hneq).
@@ -86,10 +110,10 @@ Proof.
 Qed.
 
 Lemma interp_table_add_bt :
-  forall E t e cs l, interp_table E t /\ interp_cnf E cs ->
+  forall E t e cs l, interp_table E t -> interp_cnf E cs ->
                      interp_table E (add_bt e cs l t).
 Proof.
-  move=> E t e cs l [[Hre Hrb] Hcs]. rewrite /interp_table /=. split; first done.
+  move=> E t e cs l [Hre Hrb] Hcs. rewrite /interp_table /=. split; first done.
   move=> e0 cs0 l0. case Heq : (e0 == e).
   - move/eqP: Heq => <-. rewrite find_bt_add_bt_eq. case=> <- _; done.
   - move/negP: Heq => Hneq. rewrite (find_bt_add_bt_neq _ _ _ Hneq). 
@@ -170,9 +194,19 @@ Definition correct (vm : vm) (t : comptable) :=
   (forall e cs ls, find_et e t = Some (cs, ls) -> enc_correct_exp e cs ls vm t)
   /\ forall e cs l, find_bt e t = Some (cs, l) -> enc_correct_bexp e cs l vm t.
 
-(* Ltac subexp_neq :=  *)
-(*   let H := fresh in  *)
-(*   move=> H; apply (f_equal QFBV.len_exp) in H; simpl in H; omega. *)
+Lemma correct_find_et :
+  forall vm t e cs ls,
+    correct vm t -> find_et e t = Some (cs, ls) -> enc_correct_exp e cs ls vm t.
+Proof. 
+  move=> vm t e cs ls [Hcre Hcrb]. by apply Hcre.
+Qed.
+
+Lemma correct_find_bt :
+  forall vm t e cs l,
+    correct vm t -> find_bt e t = Some (cs, l) -> enc_correct_bexp e cs l vm t.
+Proof. 
+  move=> vm t e cs l [Hcre Hcrb]. by apply Hcrb.
+Qed.
 
 Ltac auto_prove_neq :=
   match goal with
@@ -186,6 +220,17 @@ Ltac auto_prove_neq :=
     |- ~ is_true (?e1 == ?e2) => 
     let Heq := fresh in
     move=> Heq; move/eqP: Heq => Heq; rewrite Heq H2 in H1; discriminate
+  | H1 : find_bt ?e1 ?c = Some _ ,
+    H2 : find_bt ?e2 ?c = None
+    |- ~ is_true (?e1 == ?e2) =>
+    let Heq := fresh in
+    move=> Heq; move/eqP: Heq => Heq; rewrite Heq H2 in H1; discriminate
+  | H1 : find_bt ?e1 ?c = None ,
+    H2 : find_bt ?e2 ?c = Some _
+    |- ~ is_true (?e1 == ?e2) => 
+    let Heq := fresh in
+    move=> Heq; move/eqP: Heq => Heq; rewrite Heq H2 in H1; discriminate
+
   end.
 
 Lemma add_et_find_none_enc_correct_exp :
@@ -240,21 +285,57 @@ Proof.
       by apply find_bt_add_et.
 Qed.
 
-Lemma add_bt_find_none_enc_correct_bexp :
-  forall e t e0 cs0 l0 vm cs l,
-    find_bt e t = None ->
-    enc_correct_bexp e0 cs0 l0 vm t ->
-    enc_correct_bexp e0 cs0 l0 vm (add_bt e cs l t).
-Proof.
-Admitted.
-
 Lemma add_bt_find_none_enc_correct_exp :
   forall e t e0 cs0 ls0 vm cs l,
     find_bt e t = None ->
     enc_correct_exp e0 cs0 ls0 vm t ->
     enc_correct_exp e0 cs0 ls0 vm (add_bt e cs l t).
 Proof.
-Admitted.
+  move=> e t e0 cs0 ls0 vm cs l Hfe.
+  case e0 => /=.
+  - done.
+  - done.
+  - move=> op e1 [cs1 [ls1 [Hfe1 Hence]]].
+    exists cs1, ls1. split; last done.
+    rewrite -Hfe1. by rewrite find_et_add_bt.
+  - move=> op e1 e2 [cs1 [ls1 [cs2 [ls2 [Hfe1 [Hfe2 Hence]]]]]].
+    exists cs1, ls1, cs2, ls2.     
+    split; last split; last done; [rewrite -Hfe1 | rewrite -Hfe2];
+      by rewrite find_et_add_bt.
+  - move=> c e1 e2 [csc [lc [cs1 [ls1 [cs2 [ls2 [Hfc [Hfe1 [Hfe2 Hence]]]]]]]]].
+    exists csc, lc, cs1, ls1, cs2, ls2.
+    repeat split; last done.
+    + rewrite -Hfc. apply find_bt_add_bt_neq. by auto_prove_neq.
+    + rewrite -Hfe1. by apply find_et_add_bt. 
+    + rewrite -Hfe2. by apply find_et_add_bt.
+Qed.
+
+Lemma add_bt_find_none_enc_correct_bexp :
+  forall e t e0 cs0 l0 vm cs l,
+    find_bt e t = None ->
+    enc_correct_bexp e0 cs0 l0 vm t ->
+    enc_correct_bexp e0 cs0 l0 vm (add_bt e cs l t).
+Proof.
+  move=> e t e0 cs0 l0 vm cs l Hfe.
+  case e0 => /=.
+  - done.
+  - done.
+  - move=> op e1 e2 [cs1 [ls1 [cs2 [ls2 [Hfe1 [Hfe2 Hence]]]]]].
+    exists cs1, ls1, cs2, ls2.     
+    split; last split; last done; [rewrite -Hfe1 | rewrite -Hfe2];
+      by rewrite find_et_add_bt.
+  - move=> e1 [cs1 [l1 [Hfe1 Hence]]].
+    exists cs1, l1. split; last done.
+    rewrite -Hfe1. apply find_bt_add_bt_neq. by auto_prove_neq. 
+  - move=> e1 e2 [cs1 [l1 [cs2 [l2 [Hfe1 [Hfe2 Hence]]]]]].
+    exists cs1, l1, cs2, l2.     
+    split; last split; last done; [rewrite -Hfe1 | rewrite -Hfe2];
+      apply find_bt_add_bt_neq; by auto_prove_neq.       
+  - move=> e1 e2 [cs1 [l1 [cs2 [l2 [Hfe1 [Hfe2 Hence]]]]]].
+    exists cs1, l1, cs2, l2.     
+    split; last split; last done; [rewrite -Hfe1 | rewrite -Hfe2];
+      apply find_bt_add_bt_neq; by auto_prove_neq.       
+Qed.
 
 Lemma correct_add_et :
   forall vm t e cs ls, 
@@ -263,17 +344,16 @@ Lemma correct_add_et :
     -> enc_correct_exp e cs ls vm t
     -> correct vm (add_et e cs ls t).
 Proof.
-  move=> vm t e cs ls [Hce Hcb] Hfe Hence. rewrite /correct /=. 
-  split. 
+  move=> vm t e cs ls Hcr Hfe Hence. split. 
   - move=> e0 cs0 ls0. case Heq : (e0 == e).
     + move/eqP: Heq => Heq. rewrite Heq find_et_add_et_eq. case=> <- <-.
       move: Hence.
       exact: add_et_find_none_enc_correct_exp.
     + move/negP: Heq => Hneq. rewrite (find_et_add_et_neq _ _ _ Hneq).
-      move=> Hfe0. move: (Hce _ _ _ Hfe0) => {Hence}.
+      move=> Hfe0. move: (correct_find_et Hcr Hfe0) => {Hence}.
       exact: add_et_find_none_enc_correct_exp.
   - move=> e0 cs0 l0 Hfe0.
-    move: (Hcb _ _ _ Hfe0) => {Hence}.
+    move: (correct_find_bt Hcr Hfe0) => {Hence}.
     exact: add_et_find_none_enc_correct_bexp.
 Qed.
 
@@ -284,17 +364,16 @@ Lemma correct_add_bt :
     -> enc_correct_bexp e cs l vm t
     -> correct vm (add_bt e cs l t).
 Proof.
-  move=> vm t e cs ls [Hce Hcb] Hfe Hence. rewrite /correct /=. 
-  split. 
+  move=> vm t e cs ls Hcr Hfe Hence. split. 
   - move=> e0 cs0 ls0 Hfe0. 
-    move: (Hce _ _ _ Hfe0) => {Hence}.
+    move: (correct_find_et Hcr Hfe0) => {Hence}.
     exact: add_bt_find_none_enc_correct_exp.
   - move=> e0 cs0 l0. case Heq : (e0 == e).
     + move/eqP: Heq => Heq. rewrite Heq find_bt_add_bt_eq. case=> <- <-. 
       move: Hence.
       exact: add_bt_find_none_enc_correct_bexp.
     + move/negP: Heq => Hneq. rewrite (find_bt_add_bt_neq _ _ _ Hneq).
-      move=> Hfe0. move: (Hcb _ _ _ Hfe0) => {Hence}.
+      move=> Hfe0. move: (correct_find_bt Hcr Hfe0) => {Hence}.
       exact: add_bt_find_none_enc_correct_bexp.
 Qed.
 
@@ -338,11 +417,80 @@ Qed.
 Lemma vm_preserve_correct :
   forall m m' t, vm_preserve m m' -> correct m t -> correct m' t.
 Proof.
-  move=> m m' c Hpmmp [Hce Hcb]. rewrite /correct. split.
-  - move=> e cs ls Hfind. move: (Hce _ _ _ Hfind) => Hencm.
+  move=> m m' c Hpmmp Hcr. split.
+  - move=> e cs ls Hfind. move: (correct_find_et Hcr Hfind) => Hencm.
     by apply: (@vm_preserve_enc_correct_exp m).
-  - move=> e cs l Hfind. move: (Hcb _ _ _ Hfind) => Hencm.
+  - move=> e cs l Hfind. move: (correct_find_bt Hcr Hfind) => Hencm.
     by apply: (@vm_preserve_enc_correct_bexp m).
+Qed.
+
+Lemma interp_table_find_et_some_correct :
+  forall m E s t e cs ls,
+    consistent m E s -> interp_lit E lit_tt
+    -> interp_table E t -> find_et e t = Some (cs, ls) 
+    -> correct m t -> enc_bits E ls (QFBV.eval_exp e s)
+  with
+    interp_table_find_bt_some_correct :
+      forall m E s t e cs l,
+        consistent m E s -> interp_lit E lit_tt
+        -> interp_table E t -> find_bt e t = Some (cs, l) 
+        -> correct m t -> enc_bit E l (QFBV.eval_bexp e s).
+Proof.
+  (* interp_table_find_et_some_correct *)
+  move=> m E s t.
+  elim => [v | bs | op e1 IH1 | op e1 IH1 e2 IH2 | b e1 IH1 e2 IH2];
+  move=> cs ls Hcon Htt HiEt Hfe Hcrmt;
+  move: (interp_table_find_et HiEt Hfe) => Hics;
+  move: (add_prelude_to Htt Hics) => {Hics} Hics.
+  - move: (correct_find_et Hcrmt Hfe) => /= Hence.
+    by apply Hence.
+  - move: (correct_find_et Hcrmt Hfe) => /= Hence.
+    by apply (Hence E s).
+  - move: (correct_find_et Hcrmt Hfe) => /= 
+      [cs1 [ls1 [Hfe1 Hence]]].
+    move: (IH1 _ _ Hcon Htt HiEt Hfe1 Hcrmt) => Henc1.
+    by apply Hence.
+  - move: (correct_find_et Hcrmt Hfe) => /= 
+      [cs1 [ls1 [cs2 [ls2 [Hfe1 [Hfe2 Hence]]]]]].
+    move: (IH1 _ _ Hcon Htt HiEt Hfe1 Hcrmt) 
+            (IH2 _ _ Hcon Htt HiEt Hfe2 Hcrmt) => Henc1 Henc2.
+    by apply Hence.
+  - move: (correct_find_et Hcrmt Hfe) => /= 
+      [csb [lb [cs1 [ls1 [cs2 [ls2 [Hfb [Hfe1 [Hfe2 Hence]]]]]]]]].
+    move: (interp_table_find_bt_some_correct _ _ _ _ _ _ _ Hcon Htt HiEt Hfb Hcrmt) 
+            (IH1 _ _ Hcon Htt HiEt Hfe1 Hcrmt) 
+            (IH2 _ _ Hcon Htt HiEt Hfe2 Hcrmt) => Hencb Henc1 Henc2.
+    by apply Hence.
+  (* interp_table_find_bt_some_correct *)
+  move=> m E s t.
+  elim => [ | | op e1 e2 | e1 IH1 | e1 IH1 e2 IH2 | e1 IH1 e2 IH2];
+  move=> cs l Hcon Htt HiEt Hfe Hcrmt;
+  move: (interp_table_find_bt HiEt Hfe) => Hics;
+  move: (add_prelude_to Htt Hics) => {Hics} Hics.
+  - move: (correct_find_bt Hcrmt Hfe) => /= Hence.
+    by apply (Hence E s).
+  - move: (correct_find_bt Hcrmt Hfe) => /= Hence.
+    by apply (Hence E s).
+  - move: (correct_find_bt Hcrmt Hfe) => /= 
+      [cs1 [ls1 [cs2 [ls2 [Hfe1 [Hfe2 Hence]]]]]].
+    move: (interp_table_find_et_some_correct _ _ _ _ _ _ _ Hcon Htt HiEt Hfe1 Hcrmt)
+          (interp_table_find_et_some_correct _ _ _ _ _ _ _ Hcon Htt HiEt Hfe2 Hcrmt)
+           => Henc1 Henc2.
+    by apply Hence.
+  - move: (correct_find_bt Hcrmt Hfe) => /= 
+      [cs1 [l1 [Hfe1 Hence]]].
+    move: (IH1 _ _ Hcon Htt HiEt Hfe1 Hcrmt) => Henc1.
+    by apply Hence.
+  - move: (correct_find_bt Hcrmt Hfe) => /= 
+      [cs1 [l1 [cs2 [l2 [Hfe1 [Hfe2 Hence]]]]]].
+    move: (IH1 _ _ Hcon Htt HiEt Hfe1 Hcrmt) 
+            (IH2 _ _ Hcon Htt HiEt Hfe2 Hcrmt) => Henc1 Henc2.
+    by apply Hence.
+  - move: (correct_find_bt Hcrmt Hfe) => /= 
+      [cs1 [l1 [cs2 [l2 [Hfe1 [Hfe2 Hence]]]]]].
+    move: (IH1 _ _ Hcon Htt HiEt Hfe1 Hcrmt) 
+            (IH2 _ _ Hcon Htt HiEt Hfe2 Hcrmt) => Henc1 Henc2.
+    by apply Hence.
 Qed.
 
 
@@ -350,49 +498,88 @@ Qed.
 
 Definition newer_than_table g (t : comptable) :=
   (forall e cs ls, find_et e t = Some (cs, ls) 
-                   -> newer_than_cnf g cs && newer_than_lits g ls)
+                   -> newer_than_cnf g cs /\ newer_than_lits g ls)
   /\ forall e cs l, find_bt e t = Some (cs, l) 
-                    -> newer_than_cnf g cs && newer_than_lit g l.
+                    -> newer_than_cnf g cs /\ newer_than_lit g l.
+
+Lemma newer_than_table_find_et :
+  forall g t e cs ls,
+    newer_than_table g t -> find_et e t = Some (cs, ls) 
+    -> newer_than_cnf g cs /\ newer_than_lits g ls.
+Proof. 
+  move=> g t e cs ls [He Hb] Hfe. exact: (He _ _ _ Hfe).
+Qed.
+
+Lemma newer_than_table_find_bt :
+  forall g t e cs l,
+    newer_than_table g t -> find_bt e t = Some (cs, l) 
+    -> newer_than_cnf g cs /\ newer_than_lit g l.
+Proof. 
+  move=> g t e cs ls [He Hb] Hfe. exact: (Hb _ _ _ Hfe).
+Qed.
+
+Lemma newer_than_table_add_et :
+  forall g t e cs ls, 
+    newer_than_table g t -> newer_than_cnf g cs -> newer_than_lits g ls 
+    -> newer_than_table g (add_et e cs ls t).
+Proof.
+  move=> g t e cs ls Hgt Hgcs Hgls. split.
+  - move=> e0 cs0 ls0. case Heq : (e0 == e).
+    + move/eqP: Heq => <-. rewrite find_et_add_et_eq. case=> <- <-. split; done.
+    + move/negP: Heq => Hneq. rewrite (find_et_add_et_neq _ _ _ Hneq).
+      move=> Hfe. exact: (newer_than_table_find_et Hgt Hfe).
+  - move=> e0 cs0 ls0. rewrite find_bt_add_et => Hfe. 
+    exact: (newer_than_table_find_bt Hgt Hfe).
+Qed.
+
+Lemma newer_than_table_add_bt :
+  forall g t e cs l, 
+    newer_than_table g t -> newer_than_cnf g cs -> newer_than_lit g l 
+    -> newer_than_table g (add_bt e cs l t).
+Proof. 
+  move=> g t e cs l Hgt Hgcs Hgl. split.
+  - move=> e0 cs0 ls0. rewrite find_et_add_bt => Hfe. 
+    exact: (newer_than_table_find_et Hgt Hfe).
+  - move=> e0 cs0 ls0. case Heq : (e0 == e).
+    + move/eqP: Heq => <-. rewrite find_bt_add_bt_eq. case=> <- <-. split; done.
+    + move/negP: Heq => Hneq. rewrite (find_bt_add_bt_neq _ _ _ Hneq).
+      move=> Hfe. exact: (newer_than_table_find_bt Hgt Hfe).
+Qed.
+
+Lemma newer_than_table_le_newer g g' t :
+  newer_than_table g t -> (g <=? g')%positive -> newer_than_table g' t.
+Proof.
+  move=> [Hnewe Hnewb] Hgg'. split.
+  - move=> e cs ls Hfind. move: (Hnewe _ _ _ Hfind) => [Hgcs Hgls].
+    move: (newer_than_cnf_le_newer Hgcs Hgg').
+    move: (newer_than_lits_le_newer Hgls Hgg'). done.
+  - move=> e cs l Hfind. move: (Hnewb _ _ _ Hfind) => [Hgcs Hgl].
+    move: (newer_than_cnf_le_newer Hgcs Hgg').
+    move: (newer_than_lit_le_newer Hgl Hgg'). done.
+Qed.
 
 Lemma env_preserve_interp_table E E' g t :
   env_preserve E E' g -> newer_than_table g t ->
   interp_table E' t <-> interp_table E t.
 Proof.
-  move=> Henv [Hge Hgb]. rewrite /interp_table. split.
-  - apply env_preserve_sym in Henv. move=> [H1 H2]. 
+  move=> Hpre Hgt. split.
+  - apply env_preserve_sym in Hpre. move=> HiEpt. 
     split; move=> e cs ls Hfind.
-    + move: (Hge _ _ _ Hfind) => /andP [Hgcs _].
-      rewrite (env_preserve_cnf Henv Hgcs). exact: (H1 _ _ _ Hfind).
-    + move: (Hgb _ _ _ Hfind) => /andP [Hgcs _].
-      rewrite (env_preserve_cnf Henv Hgcs). exact: (H2 _ _ _ Hfind).
-  - move=> [H1 H2]. 
+    + move: (newer_than_table_find_et Hgt Hfind) => [Hgcs _].
+      rewrite (env_preserve_cnf Hpre Hgcs). 
+      exact: (interp_table_find_et HiEpt Hfind).
+    + move: (newer_than_table_find_bt Hgt Hfind) => [Hgcs _].
+      rewrite (env_preserve_cnf Hpre Hgcs). 
+      exact: (interp_table_find_bt HiEpt Hfind).
+  - move=> HiEpt. 
     split; move=> e cs ls Hfind.
-    + move: (Hge _ _ _ Hfind) => /andP [Hgcs _].
-      rewrite (env_preserve_cnf Henv Hgcs). exact: (H1 _ _ _ Hfind).
-    + move: (Hgb _ _ _ Hfind) => /andP [Hgcs _].
-      rewrite (env_preserve_cnf Henv Hgcs). exact: (H2 _ _ _ Hfind).
-Qed.    
-
-(*
-Lemma env_preserve_correct E E' s g ca :
-  env_preserve E E' g -> newer_than_cache g ca ->
-  correct E' s ca <-> correct E s ca.
-Proof.
-  move=> Henv [Hge Hgb]. rewrite /correct. split.
-  - apply env_preserve_sym in Henv. move=> [H1 H2]. 
-    split; move=> e cs ls Hfind.
-    + move: (Hge _ _ _ Hfind) => /andP [_ Hgls].
-      apply (env_preserve_enc_bits Henv Hgls). exact: (H1 _ _ _ Hfind).
-    + move: (Hgb _ _ _ Hfind) => /andP [_ Hgls].
-      apply (env_preserve_enc_bit Henv Hgls). exact: (H2 _ _ _ Hfind).
-  - move=> [H1 H2]. 
-    split; move=> e cs ls Hfind.
-    + move: (Hge _ _ _ Hfind) => /andP [_ Hgls].
-      apply (env_preserve_enc_bits Henv Hgls). exact: (H1 _ _ _ Hfind).
-    + move: (Hgb _ _ _ Hfind) => /andP [_ Hgls].
-      apply (env_preserve_enc_bit Henv Hgls). exact: (H2 _ _ _ Hfind).
-Qed.    
-*)
+    + move: (newer_than_table_find_et Hgt Hfind) => [Hgcs _].
+      rewrite (env_preserve_cnf Hpre Hgcs). 
+      exact: (interp_table_find_et HiEpt Hfind).
+    + move: (newer_than_table_find_bt Hgt Hfind) => [Hgcs _].
+      rewrite (env_preserve_cnf Hpre Hgcs). 
+      exact: (interp_table_find_bt HiEpt Hfind).
+Qed.
 
 
 (* ==== bound by vm ==== *)
@@ -401,36 +588,60 @@ Definition bound (t : comptable) (vm : vm) :=
   (forall e cs ls, find_et e t = Some (cs, ls) -> bound_exp e vm)
   /\ forall e cs l, find_bt e t = Some (cs, l) -> bound_bexp e vm.
 
+Lemma bound_find_et :
+  forall t m e cs ls, 
+    bound t m -> find_et e t = Some (cs, ls) -> bound_exp e m.
+Proof. 
+  move=> t m e cs ls [Hbe Hbb]. exact: Hbe.
+Qed.
+
+Lemma bound_find_bt :
+  forall t m e cs l, 
+    bound t m -> find_bt e t = Some (cs, l) -> bound_bexp e m.
+Proof. 
+  move=> t m e cs ls [Hbe Hbb]. exact: Hbb.
+Qed.
+
 Lemma bound_add_et :
-  forall t vm e cs ls, bound t vm /\ bound_exp e vm -> bound (add_et e cs ls t) vm.
+  forall t vm e cs ls, bound t vm -> bound_exp e vm -> bound (add_et e cs ls t) vm.
 Proof.
-  move=> t vm e cs ls [[Hbe Hbb] Hbnde]. rewrite /bound /=. split; last done.
+  move=> t vm e cs ls [Hbe Hbb] Hbnde. split; last done.
   move=> e0 cs0 ls0. case Heq : (e0 == e).
   - move/eqP: Heq => ->. done. 
   - move/negP: Heq => Hneq. rewrite (find_et_add_et_neq _ _ _ Hneq). exact: Hbe.
 Qed.
 
 Lemma bound_add_bt :
-  forall t vm e cs l, bound t vm /\ bound_bexp e vm -> bound (add_bt e cs l t) vm.
+  forall t vm e cs l, bound t vm -> bound_bexp e vm -> bound (add_bt e cs l t) vm.
 Proof.
-  move=> t vm e cs l [[Hbe Hbb] Hbnde]. rewrite /bound /=. split; first done.
+  move=> t vm e cs l [Hbe Hbb] Hbnde. split; first done.
   move=> e0 cs0 l0. case Heq : (e0 == e).
   - move/eqP: Heq => ->. done.
   - move/negP: Heq => Hneq. rewrite (find_bt_add_bt_neq _ _ _ Hneq). exact: Hbb.
 Qed.
 
-Lemma bound_add_find_none :
-  forall t vm v ls,
-    bound t vm -> SSAVM.find v vm = None -> bound t (SSAVM.add v ls vm).
+Lemma vm_preserve_bound :
+  forall m m' t, vm_preserve m m' -> bound t m -> bound t m'.
 Proof.
-  move=> t vm v ls [Hbe Hbb] Hfind. 
-  move: (vm_preserve_add_diag ls Hfind) => Hpre.
-  split. 
-  - move=> e0 cs0 ls0 Hfet. move: (Hbe _ _ _ Hfet) => Hbvm.
-    exact: (vm_preserve_bound_exp Hbvm Hpre).
-  - move=> e0 cs0 l0 Hfbt. move: (Hbb _ _ _ Hfbt) => Hbvm.
-    exact: (vm_preserve_bound_bexp Hbvm Hpre).
+  move=> m m' t Hpre [Hbe Hbb]. split.
+  - move=> e cs ls Hfind. move: (Hbe _ _ _ Hfind) => Hbdm.
+    exact: (vm_preserve_bound_exp Hbdm Hpre).
+  - move=> e cs l Hfind. move: (Hbb _ _ _ Hfind) => Hbdm.
+    exact: (vm_preserve_bound_bexp Hbdm Hpre).
 Qed.
+
+(* Lemma bound_add_find_none : *)
+(*   forall t vm v ls, *)
+(*     bound t vm -> SSAVM.find v vm = None -> bound t (SSAVM.add v ls vm). *)
+(* Proof. *)
+(*   move=> t vm v ls [Hbe Hbb] Hfind.  *)
+(*   move: (vm_preserve_add_diag ls Hfind) => Hpre. *)
+(*   split.  *)
+(*   - move=> e0 cs0 ls0 Hfet. move: (Hbe _ _ _ Hfet) => Hbvm. *)
+(*     exact: (vm_preserve_bound_exp Hbvm Hpre). *)
+(*   - move=> e0 cs0 l0 Hfbt. move: (Hbb _ _ _ Hfbt) => Hbvm. *)
+(*     exact: (vm_preserve_bound_bexp Hbvm Hpre). *)
+(* Qed. *)
 
 
 (* ==== CompTable preserve ==== *)
@@ -438,3 +649,56 @@ Qed.
 Definition preserve (t t' : comptable) : Prop :=
   (forall e cs ls, find_et e t = Some (cs, ls) -> find_et e t' = Some (cs, ls))
   /\ forall e cs l, find_bt e t = Some (cs, l) -> find_bt e t' = Some (cs, l).
+
+Lemma preserve_refl : forall t, preserve t t.
+Proof.
+  done.
+Qed.
+
+Lemma preserve_trans :
+  forall t1 t2 t3, preserve t1 t2 -> preserve t2 t3 -> preserve t1 t3.
+Proof. 
+  move=> t1 t2 t3 [Hpe12 Hpb12] [Hpe23 Hpb23]. split.
+  - move=> e cs ls Hf1. move: (Hpe12 _ _ _ Hf1). exact: Hpe23.
+  - move=> e cs l Hf1. move: (Hpb12 _ _ _ Hf1). exact: Hpb23.
+Qed.
+
+Lemma preserve_find_et :
+  forall t t' e cs ls,
+    preserve t t' -> 
+    find_et e t = Some (cs, ls) -> find_et e t' = Some (cs, ls).
+Proof.
+  move=> t t' e cs ls [Hpe Hpb]. exact: Hpe.
+Qed.
+
+Lemma preserve_find_bt :
+  forall t t' e cs l,
+    preserve t t' -> 
+    find_bt e t = Some (cs, l) -> find_bt e t' = Some (cs, l).
+Proof.
+  move=> t t' e cs ls [Hpe Hpb]. exact: Hpb.
+Qed.
+
+Lemma preserve_add_et :
+  forall t1 t2 e cs ls,
+    preserve t1 t2 -> find_et e t2 = None -> preserve t1 (add_et e cs ls t2).
+Proof. 
+  move=> t1 t2 e cs ls Hpre Hfe. split.
+  - move=> e0 cs0 ls0 Hfe0. move: (preserve_find_et Hpre Hfe0) => {Hfe0} Hfe0.
+    have Hneq : ~ (e0 == e) by auto_prove_neq.
+    rewrite (find_et_add_et_neq _ _ _ Hneq). done.
+  - move=> e0 cs0 l0 Hfe0. move: (preserve_find_bt Hpre Hfe0) => {Hfe0} Hfe0.
+    by rewrite find_bt_add_et.
+Qed.
+
+Lemma preserve_add_bt :
+  forall t1 t2 e cs l,
+    preserve t1 t2 -> find_bt e t2 = None -> preserve t1 (add_bt e cs l t2).
+Proof. 
+  move=> t1 t2 e cs l Hpre Hfe. split.
+  - move=> e0 cs0 ls0 Hfe0. move: (preserve_find_et Hpre Hfe0) => {Hfe0} Hfe0.
+    by rewrite find_et_add_bt.
+  - move=> e0 cs0 l0 Hfe0. move: (preserve_find_bt Hpre Hfe0) => {Hfe0} Hfe0.
+    have Hneq : ~ (e0 == e) by auto_prove_neq.
+    rewrite (find_bt_add_bt_neq _ _ _ Hneq). done.
+Qed.
