src/newBBCache/SimpCache.v
@@ -8,13 +8,6 @@ Set Implicit Arguments.
 Unset Strict Implicit.
 Import Prenex Implicits.
 
-(* Module ExpMap <: SsrFMap := FMaps.MakeTreeMap QFBV.ExpOrder. *)
-(* Module BexpMap <: SsrFMap := FMaps.MakeTreeMap QFBV.BexpOrder. *)
-
-(* Definition cexpm := ExpMap.t (cnf * word). *)
-(* Definition cbexpm := BexpMap.t (cnf * literal). *)
-(* Definition hexpm := ExpMap.t (cnf * word). *)
-(* Definition hbexpm := BexpMap.t (cnf * literal). *)
 
 (* ==== A cache with partial information in current tables ==== *)
 
@@ -24,100 +17,133 @@ Record cache :=
     (* store current results *)
     ct : simptable }.
 
+Definition empty : cache :=
+  {| ht := CompTable.empty;
+     ct := SimpTable.empty |}.
+
 Definition find_het e c := CompTable.find_et e (ht c).
 Definition find_hbt e c := CompTable.find_bt e (ht c). 
 Definition find_cet e c := SimpTable.find_et e (ct c). 
 Definition find_cbt e c := SimpTable.find_bt e (ct c). 
 
+
+(* ==== modification ==== *)
+
 Definition add_het e cs ls c := 
   {| ht := CompTable.add_et e cs ls (ht c);
      ct := ct c |}.
+
 Definition add_hbt e cs l c := 
   {| ht := CompTable.add_bt e cs l (ht c);
      ct := ct c |}.
+
 Definition add_cet e ls c := 
   {| ht := ht c;
      ct := SimpTable.add_et e ls (ct c) |}.
+
 Definition add_cbt e l c := 
   {| ht := ht c;
      ct := SimpTable.add_bt e l (ct c) |}.
 
 Definition reset_ct (c : cache) :=
   {| ht := ht c;
-     ct := {| et := ExpMap.empty word;
-              bt := BexpMap.empty literal |} |}.
+     ct := SimpTable.empty |}.
 
-Definition compatible_et (st : simptable) (ct : comptable) :=
-  (forall e ls, find_et e st = Some ls 
-                -> exists cs, CompTable.find_et e ct = Some (cs, ls))
-  /\ forall e cs ls, CompTable.find_et e ct = Some (cs, ls) 
-                     -> find_et e st = Some ls.
+(* Definition compatible_et (st : simptable) (ct : comptable) := *)
+(*   (forall e ls, find_et e st = Some ls  *)
+(*                 -> exists cs, CompTable.find_et e ct = Some (cs, ls)) *)
+(*   /\ forall e cs ls, CompTable.find_et e ct = Some (cs, ls)  *)
+(*                      -> find_et e st = Some ls. *)
 
-Definition compatible_bt (st : simptable) (ct : comptable) :=
-  (forall e l, find_bt e st = Some l
-               -> exists cs, CompTable.find_bt e ct = Some (cs, l))
-  /\ forall e cs l, CompTable.find_bt e ct = Some (cs, l) 
-                     -> find_bt e st = Some l.
+(* Definition compatible_bt (st : simptable) (ct : comptable) := *)
+(*   (forall e l, find_bt e st = Some l *)
+(*                -> exists cs, CompTable.find_bt e ct = Some (cs, l)) *)
+(*   /\ forall e cs l, CompTable.find_bt e ct = Some (cs, l)  *)
+(*                      -> find_bt e st = Some l. *)
+
+(* ==== compatible ==== *)
 
 Definition compatible (c1 : cache) (c2 : compcache) :=
-  SimpTable.compatible (ct c1) (CompCache.ct c2) /\ (ht c1) = (CompCache.ht c2).
+  SimpTable.compatible (ct c1) (CompCache.ct c2) 
+  /\ (ht c1) = (CompCache.ht c2).
 
+Lemma compatible_find_het :
+  forall c1 c2 e, compatible c1 c2 -> find_het e c1 = CompCache.find_het e c2.
+Proof. 
+  move=> c1 c2 e [Hct Hht] /=. rewrite /find_het Hht. done.
+Qed.
+
+Lemma compatible_find_hbt :
+  forall c1 c2 e, compatible c1 c2 -> find_hbt e c1 = CompCache.find_hbt e c2.
+Proof.
+  move=> c1 c2 e [Hct Hht] /=. rewrite /find_hbt Hht. done.
+Qed.
 
 Lemma compatible_find_cet_some :
   forall c1 c2 e ls,
     compatible c1 c2 -> find_cet e c1 = Some ls 
     -> exists cs, CompCache.find_cet e c2 = Some (cs, ls).
-Proof. Admitted.
+Proof. 
+  move=> c1 c2 e ls [Hct Hht] /=. exact: SimpTable.compatible_find_et_some.
+Qed.
 
 Lemma compatible_find_cet_none :
   forall c1 c2 e,
     compatible c1 c2 -> find_cet e c1 = None -> CompCache.find_cet e c2 = None.
-Proof. Admitted.
-
-Lemma compatible_find_het :
-  forall c1 c2 e, compatible c1 c2 -> find_het e c1 = CompCache.find_het e c2.
-Proof. Admitted.
-
-Lemma compatible_add_cet :
-  forall c1 c2 e cs ls,
-    compatible c1 c2 -> compatible (add_cet e ls c1) (CompCache.add_cet e cs ls c2).
-Proof. Admitted.
-
-Lemma compatible_add_het :
-  forall c1 c2 e cs ls,
-    compatible c1 c2 
-    -> compatible (add_het e cs ls c1) (CompCache.add_het e cs ls c2).
-Proof. Admitted.
+Proof.
+  move=> c1 c2 e [Hct Hht] /=. exact: SimpTable.compatible_find_et_none.
+Qed.
 
 Lemma compatible_find_cbt_some :
   forall c1 c2 e l,
     compatible c1 c2 -> find_cbt e c1 = Some l 
     -> exists cs, CompCache.find_cbt e c2 = Some (cs, l).
-Proof. Admitted.
+Proof.
+  move=> c1 c2 e l [Hct Hht] /=. exact: SimpTable.compatible_find_bt_some.
+Qed.
 
 Lemma compatible_find_cbt_none :
   forall c1 c2 e,
     compatible c1 c2 -> find_cbt e c1 = None -> CompCache.find_cbt e c2 = None.
-Proof. Admitted.
+Proof.
+  move=> c1 c2 e [Hct Hht] /=. exact: SimpTable.compatible_find_bt_none.
+Qed.
 
-Lemma compatible_find_hbt :
-  forall c1 c2 e, compatible c1 c2 -> find_hbt e c1 = CompCache.find_hbt e c2.
-Proof. Admitted.
-
-Lemma compatible_add_cbt :
-  forall c1 c2 e cs l,
-    compatible c1 c2 -> compatible (add_cbt e l c1) (CompCache.add_cbt e cs l c2).
-Proof. Admitted.
+Lemma compatible_add_het :
+  forall c1 c2 e cs ls,
+    compatible c1 c2 
+    -> compatible (add_het e cs ls c1) (CompCache.add_het e cs ls c2).
+Proof.
+  move=> c1 c2 e cs ls [Hct Hht]. split; [ done | by rewrite /add_het Hht ].
+Qed.
 
 Lemma compatible_add_hbt :
   forall c1 c2 e cs l,
     compatible c1 c2 
     -> compatible (add_hbt e cs l c1) (CompCache.add_hbt e cs l c2).
-Proof. Admitted.
+Proof.
+  move=> c1 c2 e cs l [Hct Hht]. split; [ done | by rewrite /add_hbt Hht ].
+Qed.
 
+Lemma compatible_add_cet :
+  forall c1 c2 e cs ls,
+    compatible c1 c2 -> compatible (add_cet e ls c1) (CompCache.add_cet e cs ls c2).
+Proof.
+  move=> c1 c2 e cs ls [Hct Hht]. 
+  split; [ exact: SimpTable.compatible_add_et | done ].
+Qed.
+
+Lemma compatible_add_cbt :
+  forall c1 c2 e cs l,
+    compatible c1 c2 -> compatible (add_cbt e l c1) (CompCache.add_cbt e cs l c2).
+Proof.
+  move=> c1 c2 e cs ls [Hct Hht]. 
+  split; [ exact: SimpTable.compatible_add_bt | done ].
+Qed.
 
 Lemma compatible_reset_ct :
-  forall c cc, compatible c cc -> compatible (SimpCache.reset_ct c) (CompCache.reset_ct cc).
-Proof. Admitted.
-
-
+  forall c1 c2, 
+    compatible c1 c2 -> compatible (reset_ct c1) (CompCache.reset_ct c2).
+Proof.
+  move=> c1 c2 [Hct Hht]. split; done.
+Qed.
